PREFIX : <https://linked.data.gov.au/def/surface-capture-method/>
PREFIX astatus: <https://linked.data.gov.au/def/reg-statuses/>
PREFIX cs: <https://linked.data.gov.au/def/surface-capture-method>
PREFIX droles: <https://linked.data.gov.au/def/data-roles/>
PREFIX owl: <http://www.w3.org/2002/07/owl#>
PREFIX prov: <http://www.w3.org/ns/prov#>
PREFIX reg: <http://purl.org/linked-data/registry#>
PREFIX schema: <https://schema.org/>
PREFIX skos: <http://www.w3.org/2004/02/skos/core#>
PREFIX unggim: <https://linked.data.gov.au/def/unggim-themes/>
PREFIX xsd: <http://www.w3.org/2001/XMLSchema#>

:imagery-auto
    a skos:Concept ;
    skos:altLabel "Imagery auto"@en ;
    skos:definition "Surface information has been automatically extracted from imagery. "@en ;
    skos:historyNote "Queensland Roads and Tracks dataset" ;
    skos:inScheme cs: ;
    skos:prefLabel "Imagery Automated"@en ;
.

:imagery-manual
    a skos:Concept ;
    skos:altLabel "Imagery manual"@en ;
    skos:definition "Surface information has been manually assessed from imagery. "@en ;
    skos:historyNote "Queensland Roads and Tracks dataset" ;
    skos:inScheme cs: ;
    skos:prefLabel "Imagery Manual"@en ;
.

:inherited
    a skos:Concept ;
    skos:definition "Surface information was inherited from a previous dataset. "@en ;
    skos:historyNote "Queensland Roads and Tracks dataset" ;
    skos:inScheme cs: ;
    skos:prefLabel "Inherited"@en ;
.

:lg
    a skos:Concept ;
    skos:altLabel "LG"@en ;
    skos:definition "Surface information has been supplied by Local Government. "@en ;
    skos:historyNote "Queensland Roads and Tracks dataset" ;
    skos:inScheme cs: ;
    skos:prefLabel "Local Government"@en ;
.

:other
    a skos:Concept ;
    skos:altLabel "Other"@en ;
    skos:definition "Surface information has come from another source. "@en ;
    skos:historyNote "Queensland Roads and Tracks dataset" ;
    skos:inScheme cs: ;
    skos:prefLabel "Other"@en ;
.

:port-authority
    a skos:Concept ;
    skos:altLabel "PA"@en ;
    skos:definition "Surface information has been supplied by a Port Authority. "@en ;
    skos:historyNote "Queensland Roads and Tracks dataset" ;
    skos:inScheme cs: ;
    skos:prefLabel "Port Authority"@en ;
.

:private-entity
    a skos:Concept ;
    skos:altLabel "PE"@en ;
    skos:definition "Surface information has been supplied by a private entity e.g. developer, land owner. "@en ;
    skos:historyNote "Queensland Roads and Tracks dataset" ;
    skos:inScheme cs: ;
    skos:prefLabel "Private Entity"@en ;
.

:qpws
    a skos:Concept ;
    skos:altLabel "QPWS"@en ;
    skos:definition "Surface information has been supplied by Queensland Parks and Wildlife Service. "@en ;
    skos:historyNote "Queensland Roads and Tracks dataset" ;
    skos:inScheme cs: ;
    skos:prefLabel "Queensland Parks and Wildlife Service"@en ;
    skos:scopeNote "Queensland only. " ;
.

:state
    a skos:Concept ;
    skos:altLabel "STATE"@en ;
    skos:definition "Surface information has been supplied by other state authority. "@en ;
    skos:historyNote "Queensland Roads and Tracks dataset" ;
    skos:inScheme cs: ;
    skos:prefLabel "State Department"@en ;
.

:tmr
    a skos:Concept ;
    skos:altLabel "TMR"@en ;
    skos:definition "Surface information has been supplied by the Queensland Department of Transport and Main Roads. "@en ;
    skos:historyNote "Queensland Roads and Tracks dataset" ;
    skos:inScheme cs: ;
    skos:prefLabel "Department of Transport and Main Roads"@en ;
    skos:scopeNote "Queensland only. " ;
.

:unknown
    a skos:Concept ;
    skos:altLabel "Unknown"@en ;
    skos:definition "Surface information source is unknown. "@en ;
    skos:historyNote "Queensland Roads and Tracks dataset" ;
    skos:inScheme cs: ;
    skos:prefLabel "Unknown"@en ;
.

:utility-provider
    a skos:Concept ;
    skos:altLabel "UP"@en ;
    skos:definition "Surface information has been supplied by a utility provider. "@en ;
    skos:historyNote "Queensland Roads and Tracks dataset" ;
    skos:inScheme cs: ;
    skos:prefLabel "Utility Provider"@en ;
.

:water-authority
    a skos:Concept ;
    skos:altLabel "WA"@en ;
    skos:definition "Surface information has been supplied by a Water Authority. "@en ;
    skos:historyNote "Queensland Roads and Tracks dataset" ;
    skos:inScheme cs: ;
    skos:prefLabel "Water Authority"@en ;
.

:1.0 schema:name "1.0" .

cs:
    a skos:ConceptScheme ;
    reg:status astatus:experimental ;
    owl:versionIRI :1.0 ;
    owl:versionInfo "1.0" ;
    skos:definition "This vocabulary describes the method in which road surface type was captured. "@en ;
    skos:hasTopConcept
        :imagery-auto ,
        :imagery-manual ,
        :inherited ,
        :lg ,
        :other ,
        :port-authority ,
        :private-entity ,
        :qpws ,
        :state ,
        :tmr ,
        :unknown ,
        :utility-provider ,
        :water-authority ;
        skos:historyNote """2025-05 NJC: Added status experimental

This vocabulary was created by the Queensland Spatial Information services.""" ;
    skos:prefLabel "Surface capture method"@en ;
    prov:qualifiedAttribution
        [
            prov:agent <https://linked.data.gov.au/org/icsm> ;
            prov:hadRole droles:custodian ;
        ] ;
    schema:creator <https://linked.data.gov.au/org/qsi> ;
    schema:dateCreated "2023-05-30"^^xsd:date ;
    schema:dateModified "2025-05-22"^^xsd:date ;
    schema:keywords unggim:TransportNetworks ;
    schema:publisher <https://linked.data.gov.au/org/icsm> ;
    schema:status <https://linked.data.gov.au/def/reg-statuses/experimental> ;
.
