PREFIX : <https://linked.data.gov.au/def/csdm/nz-vector-purpose/>
PREFIX cs: <https://linked.data.gov.au/def/csdm/nz-vector-purpose>
PREFIX dct: <http://purl.org/dc/terms/>
PREFIX prov: <http://www.w3.org/ns/prov#>
PREFIX rdfs: <http://www.w3.org/2000/01/rdf-schema#>
PREFIX schema: <https://schema.org/>
PREFIX skos: <http://www.w3.org/2004/02/skos/core#>
PREFIX termtype: <https://linked.data.gov.au/def/csdm/termtypes/>
PREFIX xsd: <http://www.w3.org/2001/XMLSchema#>

:adopted
    a
        skos:Concept ,
        termtype:VectorPurpose ;
    skos:definition "The dimensions of the observation were adopted from a previous survey where the dimensions had been measured" ;
    skos:inScheme cs: ;
    skos:notation "adopted" ;
    skos:prefLabel "adopted" ;
    skos:topConceptOf cs: ;
.

:calculated
    a
        skos:Concept ,
        termtype:VectorPurpose ;
    skos:definition "The dimensions of the observation where calculated" ;
    skos:inScheme cs: ;
    skos:notation "calculated" ;
    skos:prefLabel "calculated" ;
    skos:topConceptOf cs: ;
.

:measured
    a
        skos:Concept ,
        termtype:VectorPurpose ;
    skos:definition "The dimensions of the observation were measured when the survey was conducted" ;
    skos:inScheme cs: ;
    skos:notation "measured" ;
    skos:prefLabel "measured" ;
    skos:topConceptOf cs: ;
.

:pseudo
    a
        skos:Concept ,
        termtype:VectorPurpose ;
    skos:definition "The dimensions of the observation were calculated by Landonline from the coordinates of the local and remote setup's" ;
    skos:inScheme cs: ;
    skos:notation "pseudo" ;
    skos:prefLabel "pseudo" ;
    skos:topConceptOf cs: ;
.

:reinadopted
    a
        skos:Concept ,
        termtype:VectorPurpose ;
    skos:altLabel "rein adopted" ;
    skos:definition "The dimensions of the observation were used for a reinstated boundary – no parcels are created" ;
    skos:inScheme cs: ;
    skos:notation "reinadopted" ;
    skos:prefLabel "reinadopted" ;
    skos:topConceptOf cs: ;
.

:reincalculated
    a
        skos:Concept ,
        termtype:VectorPurpose ;
    skos:altLabel "rein calculated" ;
    skos:definition "The dimensions of the observation were used for a reinstated boundary – no parcels are created" ;
    skos:inScheme cs: ;
    skos:notation "reincalculated" ;
    skos:prefLabel "reincalculated" ;
    skos:topConceptOf cs: ;
.

:scaled
    a
        skos:Concept ,
        termtype:VectorPurpose ;
    skos:altLabel "calculated" ;
    skos:definition "The dimensions of the observation were scaled from a graphical plot" ;
    skos:inScheme cs: ;
    skos:notation "scaled" ;
    skos:prefLabel "scaled" ;
    skos:topConceptOf cs: ;
.

<https://linked.data.gov.au/org/csdm-pg>
    a schema:Organization ;
    schema:name "CSDM Project Group" ;
    schema:parentOrganization <https://linked.data.gov.au/org/icsm> ;
    schema:url "https://icsm-au.github.io/3d-csdm/docs/"^^xsd:anyURI ;
.

<https://linked.data.gov.au/org/icsm>
    a schema:Organization ;
    schema:name "Intergovernmental Committee on Surveying & Mapping" ;
    schema:url "https://icsm.gov.au"^^xsd:anyURI ;
.

cs:
    a skos:ConceptScheme ;
    skos:definition "NZ Vector Purpose"@en ;
    skos:hasTopConcept
        :adopted ,
        :calculated ,
        :measured ,
        :pseudo ,
        :reinadopted ,
        :reincalculated ,
        :scaled ;
    skos:prefLabel "NZ Vector Purpose" ;
    skos:scopeNote "termtype:VectorPurpose" ;
    schema:creator <https://linked.data.gov.au/org/csdm-pg> ;
    schema:dateCreated "2022-03-18"^^xsd:date ;
    schema:dateModified "2024-04-11"^^xsd:date ;
    schema:publisher <https://linked.data.gov.au/org/icsm> ;
.

[]    a prov:Activity ;
    prov:endedAtTime "2024-04-11T06:11:33.732587"^^xsd:dateTime ;
    prov:startedAtTime "2024-04-11T06:11:33.664072"^^xsd:dateTime ;
    prov:used
        [
            a prov:Entity ;
            dct:format "application/json" ;
            dct:hasVersion "git:29bbdd91c50914400e0758872364ec1cea2d1501" ;
            rdfs:seeAlso <file:///home/runner/work/icsm-vocabs/icsm-vocabs/cadastre/SurveyObservations/nz-vector-purpose.csv> ;
        ] ;
    prov:wasAssociatedWith
        [
            a
                prov:Agent ,
                schema:SoftwareApplication ;
            rdfs:label "OGC-NA tools" ;
            dct:hasVersion "0.3.44" ;
            rdfs:seeAlso <https://github.com/opengeospatial/ogc-na-tools> ;
        ] ;
    prov:wasInformedBy
        [
            dct:identifier "42611fe7-ad51-40e1-adf8-e3a0f1ee7a83" ;
        ] ; ;
.
