PREFIX : <https://linked.data.gov.au/def/csdm/icsm-admin-unit-type/>
PREFIX cs: <https://linked.data.gov.au/def/csdm/icsm-admin-unit-type>
PREFIX dcterms: <http://purl.org/dc/terms/>
PREFIX prov: <http://www.w3.org/ns/prov#>
PREFIX rdfs: <http://www.w3.org/2000/01/rdf-schema#>
PREFIX schema: <https://schema.org/>
PREFIX skos: <http://www.w3.org/2004/02/skos/core#>
PREFIX termtype: <https://linked.data.gov.au/def/csdm/termtypes/>
PREFIX unggim: <https://linked.data.gov.au/def/unggim-themes/>
PREFIX xsd: <http://www.w3.org/2001/XMLSchema#>

:county
    a
        skos:Concept ,
        termtype:AdminUnitType ;
    skos:definition "A Victorian cadastral division for cadastral or land administration purposes" ;
    skos:inScheme cs: ;
    skos:notation "county" ;
    skos:prefLabel "County" ;
    skos:topConceptOf cs: ;
.

:landDistrict
    a
        skos:Concept ,
        termtype:AdminUnitType ;
    skos:definition "A Land District is a NZ administrative area that all titles and surveys were registered against prior to Landonline." ;
    skos:inScheme cs: ;
    skos:notation "landDistrict" ;
    skos:prefLabel "Land District" ;
    skos:topConceptOf cs: ;
.

:localGovernmentArea
    a
        skos:Concept ,
        termtype:AdminUnitType ;
    skos:altLabel "Local Government" ;
    skos:definition "Local government is the third level of government in Australia, administered with limited autonomy under the states and territories, and in turn beneath the federal government" ;
    skos:inScheme cs: ;
    skos:notation "localGovernmentArea" ;
    skos:prefLabel "Local Government Area" ;
    skos:topConceptOf cs: ;
.

:locality
    a
        skos:Concept ,
        termtype:AdminUnitType ;
    skos:definition "A subdivision of a Western Australian Local Government Area" ;
    skos:inScheme cs: ;
    skos:notation "locality" ;
    skos:prefLabel "Locality" ;
    skos:topConceptOf cs: ;
.

:parish
    a
        skos:Concept ,
        termtype:AdminUnitType ;
    skos:definition "A subdivision of a Victorian County" ;
    skos:inScheme cs: ;
    skos:notation "parish" ;
    skos:prefLabel "Parish" ;
    skos:topConceptOf cs: ;
.

:territorialAuthority
    a
        skos:Concept ,
        termtype:AdminUnitType ;
    skos:altLabel "Municipality" ;
    skos:definition "A NZ territorial authority is defined under the Local Government Act 2002, NZ, as a city or a district council" ;
    skos:inScheme cs: ;
    skos:notation "territorialAuthority" ;
    skos:prefLabel "Territorial Authority" ;
    skos:topConceptOf cs: ;
.

<https://linked.data.gov.au/org/csdm-pg>
    a schema:Organization ;
    schema:name "CSDM Project Group" ;
    schema:parentOrganization <https://linked.data.gov.au/org/icsm> ;
    schema:url "https://icsm-au.github.io/3d-csdm/docs/"^^xsd:anyURI ;
.

cs:
    a skos:ConceptScheme ;
    skos:definition "ICSM Administrative Unit Types"@en ;
    skos:hasTopConcept
        :county ,
        :landDistrict ,
        :localGovernmentArea ,
        :locality ,
        :parish ,
        :territorialAuthority ;
    skos:prefLabel "ICSM Administrative Unit Types" ;
    skos:scopeNote "termtype:AdminUnitType" ;
    schema:creator <https://linked.data.gov.au/org/csdm-pg> ;
    schema:dateCreated "2022-03-18"^^xsd:date ;
    schema:dateModified "2024-08-20"^^xsd:date ;
    schema:keywords unggim:LandParcels ;
    schema:publisher <https://linked.data.gov.au/org/icsm> ;
.

[]    a prov:Activity ;
    prov:endedAtTime "2024-04-11T06:11:41.832340"^^xsd:dateTime ;
    prov:startedAtTime "2024-04-11T06:11:41.764171"^^xsd:dateTime ;
    prov:used
        [
            a prov:Entity ;
            dcterms:format "application/json" ;
            dcterms:hasVersion "git:29bbdd91c50914400e0758872364ec1cea2d1501" ;
            rdfs:seeAlso "file:///home/runner/work/icsm-vocabs/icsm-vocabs/cadastre/CSD-Header/icsm-admin-unit-type.csv" ;
        ] ;
    prov:wasAssociatedWith
        [
            a
                prov:Agent ,
                schema:SoftwareApplication ;
            rdfs:label "OGC-NA tools" ;
            dcterms:hasVersion "0.3.44" ;
            rdfs:seeAlso "https://github.com/opengeospatial/ogc-na-tools" ;
        ] ;
    prov:wasInformedBy
        [
            dcterms:identifier "42611fe7-ad51-40e1-adf8-e3a0f1ee7a83" ;
        ] ; ;
.
