PREFIX : <https://linked.data.gov.au/def/csdm/nz-survey-purpose/>
PREFIX cs: <https://linked.data.gov.au/def/csdm/nz-survey-purpose>
PREFIX dct: <http://purl.org/dc/terms/>
PREFIX prov: <http://www.w3.org/ns/prov#>
PREFIX rdfs: <http://www.w3.org/2000/01/rdf-schema#>
PREFIX schema: <https://schema.org/>
PREFIX skos: <http://www.w3.org/2004/02/skos/core#>
PREFIX surv: <https://linked.data.gov.au/def/csdm/surveyfeatures/>
PREFIX unggim: <https://linked.data.gov.au/def/unggim-themes/>
PREFIX xsd: <http://www.w3.org/2001/XMLSchema#>

:amalgamation
    a
        skos:Concept ,
        surv:SurveyPurpose ;
    skos:definition "To be used to depict amalgamations of Māori land Blocks. Survey system information may be adopted by other surveys. Tenure system information may be used to define interests in all land tenures. " ;
    skos:inScheme cs: ;
    skos:notation "amalgamation" ;
    skos:prefLabel "Amalgamations" ;
    skos:topConceptOf cs: ;
.

:application
    a
        skos:Concept ,
        surv:SurveyPurpose ;
    skos:definition "To be used when registering land under the Land Transfer Act for the first time – usually from Deeds Registered land. Includes Adverse Possession under the Land Transfer Amendment Act 1963. Application for Accretion. Survey system information may be adopted by other surveys. Tenure system information may be used to define interests in all land tenures." ;
    skos:inScheme cs: ;
    skos:notation "application" ;
    skos:prefLabel "Application" ;
    skos:topConceptOf cs: ;
.

:cbr
    a
        skos:Concept ,
        surv:SurveyPurpose ;
    skos:definition "Used to record one or more boundary marks when the boundary points are not required by the Cadastral Survey Rules 2021. Survey system information may be adopted by other surveys. Tenure system information may be used to define interests in all land tenures." ;
    skos:inScheme cs: ;
    skos:notation "cbr" ;
    skos:prefLabel "Complex Boundary Reinstatement" ;
    skos:topConceptOf cs: ;
.

:ce
    a
        skos:Concept ,
        surv:SurveyPurpose ;
    skos:definition "To be used to depict areas of land of customary entitlement (other than Nohoanga (campsite) sites) in Māori Claim Settlement legislation. Survey system information may be adopted by other surveys. Tenure system information may be used to define interests in Customary Entitlement sites only." ;
    skos:inScheme cs: ;
    skos:notation "ce" ;
    skos:prefLabel "Customary Entitlement" ;
    skos:topConceptOf cs: ;
.

:cfl
    a
        skos:Concept ,
        surv:SurveyPurpose ;
    skos:definition "To be used to depict Crown Forest License areas. Note: to be recorded in terms of OSG Policy 1997/01. Survey system information may be adopted by other surveys. Tenure system information may be used to define interests in crown forest licenses only. " ;
    skos:inScheme cs: ;
    skos:notation "cfl" ;
    skos:prefLabel "Crown Forest Lease" ;
    skos:topConceptOf cs: ;
.

:consolidation
    a
        skos:Concept ,
        surv:SurveyPurpose ;
    skos:definition "To be used to depict consolidations of Māori land Blocks. Survey system information may be adopted by other surveys. Tenure system information may be used to define interests in all land tenures. " ;
    skos:inScheme cs: ;
    skos:notation "consolidation" ;
    skos:prefLabel "Consolidations" ;
    skos:topConceptOf cs: ;
.

:csp
    a
        skos:Concept ,
        surv:SurveyPurpose ;
    skos:definition "To be used to depict subdivisions of Crown land. Includes definition of a single Crown land parcel. Survey system information may be adopted by other surveys. Tenure system information may be used to define interests in all land tenures. " ;
    skos:inScheme cs: ;
    skos:notation "csp" ;
    skos:prefLabel "Crown Subdivision Plan" ;
    skos:topConceptOf cs: ;
.

:csup
    a
        skos:Concept ,
        surv:SurveyPurpose ;
    skos:definition "To depict a complete Unit Title staged development CSD produced under the Unit Titles Act 1972 and the Unit Titles Amendment Act 1979. No survey system information is provided. Tenure system information may be used, or adopted for use, in defining applicable interests in unit tenures." ;
    skos:inScheme cs: ;
    skos:notation "csup" ;
    skos:prefLabel "Complete Stage Unit Plan" ;
    skos:topConceptOf cs: ;
.

:csup-ss
    a
        skos:Concept ,
        surv:SurveyPurpose ;
    skos:definition "To depict a complete Unit Title staged development CSD with survey sheet produced under the Unit Titles Act 1972 and the Unit Titles Amendment Act 1979. Survey system information may be adopted by other surveys. Tenure system information may be used to define interests in units, easements or covenants only." ;
    skos:inScheme cs: ;
    skos:notation "csup-ss" ;
    skos:prefLabel "Complete Stage Unit Plan with Survey Sheet" ;
    skos:topConceptOf cs: ;
.

:easement
    a
        skos:Concept ,
        surv:SurveyPurpose ;
    skos:definition "To be used for depicting an easement when it is not part of a current land subdivision survey. Includes survey of Profit-a-Prendre and Esplanade Strips. Survey system information may be adopted by other surveys. Tenure system information may be used to define interests in easements only. " ;
    skos:inScheme cs: ;
    skos:notation "easement" ;
    skos:prefLabel "Easement" ;
    skos:topConceptOf cs: ;
.

:fpcp
    a
        skos:Concept ,
        surv:SurveyPurpose ;
    skos:definition "To depict a standard CSD that shows Flats or Cross Leases. Survey of Restrictive Covenant areas only. No survey system information is provided. Tenure system information may be used to define interests in flat and cross lease parcels only. " ;
    skos:inScheme cs: ;
    skos:notation "fpcp" ;
    skos:prefLabel "Flat plan/Crosslease Plan" ;
    skos:topConceptOf cs: ;
.

:fpcp-ss
    a
        skos:Concept ,
        surv:SurveyPurpose ;
    skos:definition "To depict a standard CSD that shows Flats or Cross Leases and Survey of Restrictive Covenant areas only that includes a survey sheet. Survey system information may be adopted by other surveys. Tenure system information may be used to define interests in flat and cross lease parcels, easements or covenants only. " ;
    skos:inScheme cs: ;
    skos:notation "fpcp-ss" ;
    skos:prefLabel "Flat plan/Crosslease with Survey Sheet" ;
    skos:topConceptOf cs: ;
.

:fsup
    a
        skos:Concept ,
        surv:SurveyPurpose ;
    skos:definition "To depict the first stage of a Unit Title staged development CSD produced under the Unit Titles Act 1972 and the Unit Titles Amendment Act 1979. No survey system information is provided. Tenure system information may be used, or adopted for use, in defining applicable interests in unit tenures." ;
    skos:inScheme cs: ;
    skos:notation "fsup" ;
    skos:prefLabel "First Stage Unit Plan" ;
    skos:topConceptOf cs: ;
.

:fsup-ss
    a
        skos:Concept ,
        surv:SurveyPurpose ;
    skos:definition "To depict the first stage of a Unit Title staged development CSD with survey sheet, produced under the Unit Titles Act 1972 and the Unit Titles Amendment Act 1979. Survey system information may be adopted by other surveys. Tenure system information may be used to define interests in units, easements or covenants only." ;
    skos:inScheme cs: ;
    skos:notation "fsup-ss" ;
    skos:prefLabel "First Stage Unit Plan with Survey Sheet" ;
    skos:topConceptOf cs: ;
.

:h-c-s
    a
        skos:Concept ,
        surv:SurveyPurpose ;
    skos:definition "Historical survey purpose - Crown Parcel Definition" ;
    skos:inScheme cs: ;
    skos:notation "h-c-s" ;
    skos:prefLabel "Crown Subdivision" ;
    skos:topConceptOf cs: ;
.

:h-cbr
    a
        skos:Concept ,
        surv:SurveyPurpose ;
    skos:definition "Historical survey purpose - Boundary Reinstatement - Full CSD" ;
    skos:inScheme cs: ;
    skos:notation "h-cbr" ;
    skos:prefLabel "Complex Boundary Reinstatement" ;
    skos:topConceptOf cs: ;
.

:h-covenant
    a
        skos:Concept ,
        surv:SurveyPurpose ;
    skos:definition "Historical survey purpose - Covenant" ;
    skos:inScheme cs: ;
    skos:notation "h-covenant" ;
    skos:prefLabel "Land Transfer Plan Land Covenant, or Survey Office Plan Land Covenant" ;
    skos:topConceptOf cs: ;
.

:h-na
    a
        skos:Concept ,
        surv:SurveyPurpose ;
    skos:definition "Historical survey purpose - Compiled Survey Information OR Offsetting (for record purposes only) OR Redefinition Record Purposes Only OR Statutory Boundary" ;
    skos:inScheme cs: ;
    skos:notation "h-na" ;
    skos:prefLabel "Not Applicable" ;
    skos:topConceptOf cs: ;
.

:h-s-i
    a
        skos:Concept ,
        surv:SurveyPurpose ;
    skos:definition "Historical survey purpose - Control OR Offsetting (for approval as to survey) OR Traverses OR Inspection" ;
    skos:inScheme cs: ;
    skos:notation "h-s-i" ;
    skos:prefLabel "Survey Information" ;
    skos:topConceptOf cs: ;
.

:h-sbr
    a
        skos:Concept ,
        surv:SurveyPurpose ;
    skos:definition "Historical survey purpose - Monumentation CSD" ;
    skos:inScheme cs: ;
    skos:notation "h-sbr" ;
    skos:prefLabel "Simple Boundary Reinstatement" ;
    skos:topConceptOf cs: ;
.

:lease
    a
        skos:Concept ,
        surv:SurveyPurpose ;
    skos:definition "To be used to depict parcels for leasehold title. These overlay but do not supersede the underlying cadastre. Survey system information may be adopted by other surveys. Tenure system information may be used to define leasehold interest in the land only." ;
    skos:inScheme cs: ;
    skos:notation "lease" ;
    skos:prefLabel "Lease" ;
    skos:topConceptOf cs: ;
.

:legalisation
    a
        skos:Concept ,
        surv:SurveyPurpose ;
    skos:definition "To be used to depict land to be taken for road or other public purpose. Also may include definition of severances or areas of road to be closed. Includes Treaty Settlement Plans. Survey system information may be adopted by other surveys. Tenure system information may be used to define interests in all land tenures." ;
    skos:inScheme cs: ;
    skos:notation "legalisation" ;
    skos:prefLabel "Legalisation" ;
    skos:topConceptOf cs: ;
.

:lt
    a
        skos:Concept ,
        surv:SurveyPurpose ;
    skos:definition "To be used to depict a definition or subdivision of land owned in fee simple when that land is held in a title Limited asto parcels. Survey system information may be adopted by other surveys. Tenure system information may be used to define interests in all land tenures. " ;
    skos:inScheme cs: ;
    skos:notation "lt" ;
    skos:prefLabel "Limited Title" ;
    skos:topConceptOf cs: ;
.

:ltlc
    a
        skos:Concept ,
        surv:SurveyPurpose ;
    skos:definition "To be used for depicting land covenants on registered land when only the covenant is shown on the plan i.e. not associated with a current land subdivision survey. Survey system information may be adopted by other surveys. Tenure system information may be used to define interests in land covenants only. " ;
    skos:inScheme cs: ;
    skos:notation "ltlc" ;
    skos:prefLabel "Land Transfer Plan Land Covenant" ;
    skos:topConceptOf cs: ;
.

:lts
    a
        skos:Concept ,
        surv:SurveyPurpose ;
    skos:definition "To be used to depict subdivisions of land owned in fee simple. Includes a new definition of a single parcel. Includes surveys of Amalgamation. Survey system information may be adopted by other surveys. Tenure system information may be used to define interests in all land tenures. " ;
    skos:inScheme cs: ;
    skos:notation "lts" ;
    skos:prefLabel "LT Subdivision" ;
    skos:topConceptOf cs: ;
.

:mf
    a
        skos:Concept ,
        surv:SurveyPurpose ;
    skos:definition "To be used to depict areas required for Marine Farming purposes. Survey system information may be adopted by other surveys. Tenure system information may be used to define interests in marine farming leases only. " ;
    skos:inScheme cs: ;
    skos:notation "mf" ;
    skos:prefLabel "Marine Farming" ;
    skos:topConceptOf cs: ;
.

:mining
    a
        skos:Concept ,
        surv:SurveyPurpose ;
    skos:definition "To be used to depict areas of land (including water) with a mining permit or license. These overlay but do not supersede the underlying cadastre. Survey system information may be adopted by other surveys. Tenure system information may be used to define interests in all land tenures. " ;
    skos:inScheme cs: ;
    skos:notation "mining" ;
    skos:prefLabel "Mining" ;
    skos:topConceptOf cs: ;
.

:n-c
    a
        skos:Concept ,
        surv:SurveyPurpose ;
    skos:definition "To be used to depict areas of land designated as Nohoanga (campsite) sites in Māori Claim Settlement legislation. Survey system information may be adopted by other surveys. Tenure system information may be used to define interests in Nohoanga sites only." ;
    skos:inScheme cs: ;
    skos:notation "n-c" ;
    skos:prefLabel "Nohoanga (Campsite)" ;
    skos:topConceptOf cs: ;
.

:partition
    a
        skos:Concept ,
        surv:SurveyPurpose ;
    skos:definition "To be used to depict partitions (subdivisions) in accordance with a Māori Land Court Partition Order. Survey system information may be adopted by other surveys. Tenure system information may be used to define interests in all land tenures." ;
    skos:inScheme cs: ;
    skos:notation "partition" ;
    skos:prefLabel "Partition" ;
    skos:topConceptOf cs: ;
.

:pud
    a
        skos:Concept ,
        surv:SurveyPurpose ;
    skos:definition "To depict a standard proposed Unit Development CSD produced under the Unit Titles Act 1972. No survey system information is provided. Tenure system information may be used, or adopted for use, in defining applicable interests in unit tenures." ;
    skos:inScheme cs: ;
    skos:notation "pud" ;
    skos:prefLabel "Proposed Unit Development" ;
    skos:topConceptOf cs: ;
.

:pud-ss
    a
        skos:Concept ,
        surv:SurveyPurpose ;
    skos:definition "To depict a proposed Unit Development plan with survey sheet produced under the Unit Titles Act 1972. Survey system information may be adopted by other surveys. Tenure system information may be used to define interests in units, easements or covenants only." ;
    skos:inScheme cs: ;
    skos:notation "pud-ss" ;
    skos:prefLabel "Proposed Unit Development with Survey Sheet" ;
    skos:topConceptOf cs: ;
.

:reclamation
    a
        skos:Concept ,
        surv:SurveyPurpose ;
    skos:definition "To be used to depict land registered under the LandTransfer Act for reclamation of seabed, foreshore, stream/riverbed, or lakebed. Survey system information may be adopted by other surveys. Tenure system information may be used to define interests in all land tenures." ;
    skos:inScheme cs: ;
    skos:notation "reclamation" ;
    skos:prefLabel "Reclamation" ;
    skos:topConceptOf cs: ;
.

:revesting
    a
        skos:Concept ,
        surv:SurveyPurpose ;
    skos:definition "To be used to depict parcels to be revested as Māori land Blocks. Survey system information may be adopted by other surveys. Tenure system information may be used to define interests in all land tenures." ;
    skos:inScheme cs: ;
    skos:notation "revesting" ;
    skos:prefLabel "Revesting" ;
    skos:topConceptOf cs: ;
.

:roadway
    a
        skos:Concept ,
        surv:SurveyPurpose ;
    skos:definition "To be used to depict roadways over Māori land. Survey system information may be adopted by other surveys. Tenure system information may be used to define interests in all land tenures. " ;
    skos:inScheme cs: ;
    skos:notation "roadway" ;
    skos:prefLabel "Roadway" ;
    skos:topConceptOf cs: ;
.

:rup
    a
        skos:Concept ,
        surv:SurveyPurpose ;
    skos:definition "To depict a redevelopment Unit Title staged development CSD produced under the Unit Titles Act 1972 and the Unit Titles Amendment Act 1979. No survey system information is provided. Tenure system information may be used, or adopted for use, in defining applicable interests in unit tenures" ;
    skos:inScheme cs: ;
    skos:notation "rup" ;
    skos:prefLabel "Redevelopment Unit Plan" ;
    skos:topConceptOf cs: ;
.

:rup-ss
    a
        skos:Concept ,
        surv:SurveyPurpose ;
    skos:definition "To depict a redevelopment Unit Title staged development CSD with survey sheet, produced under the Unit Titles Act 1972 and the Unit Titles Amendment Act 1979. Survey system information may be adopted by other surveys. Tenure system information may be used to define interests in units, easements or covenants only." ;
    skos:inScheme cs: ;
    skos:notation "rup-ss" ;
    skos:prefLabel "Redevelopment Unit Plan with Survey Sheet" ;
    skos:topConceptOf cs: ;
.

:sbr
    a
        skos:Concept ,
        surv:SurveyPurpose ;
    skos:definition "Used to record the placement of one or more boundary marks on an existing boundary point in accordance with Cadastral Survey Rules 2021. Mandatory supporting document (survey report) is to be attached. Survey system information may be adopted by other surveys. Tenure system information may be used to define interests in all land tenures." ;
    skos:inScheme cs: ;
    skos:notation "sbr" ;
    skos:prefLabel "Simple Boundary Reinstatement" ;
    skos:topConceptOf cs: ;
.

:se-r
    a
        skos:Concept ,
        surv:SurveyPurpose ;
    skos:definition "To be used for depicting a statutory easement or right when it is not part of a current land subdivision survey. Includes plans of Marginal Strips. Survey system information may be adopted by other surveys. Tenure system information may be used to define interests in statutory easements or rights only. " ;
    skos:inScheme cs: ;
    skos:notation "se-r" ;
    skos:prefLabel "Statutory Easement/Right" ;
    skos:topConceptOf cs: ;
.

:si
    a
        skos:Concept ,
        surv:SurveyPurpose ;
    skos:definition "To depict survey work which does not define parcels. Survey system information may be adopted by other surveys. These surveys contain no tenure system information. " ;
    skos:inScheme cs: ;
    skos:notation "si" ;
    skos:prefLabel "Survey Information" ;
    skos:topConceptOf cs: ;
.

:soplc
    a
        skos:Concept ,
        surv:SurveyPurpose ;
    skos:definition "To be used for depicting land covenants over unregistered land when only the covenant is shown on the plan (ie not associated with a current land subdivision survey) Survey system information may be adopted by other surveys. Tenure system information may be used to define interests in land covenants only. . " ;
    skos:inScheme cs: ;
    skos:notation "soplc" ;
    skos:prefLabel "Survey Office Plan Land Covenant" ;
    skos:topConceptOf cs: ;
.

:spud
    a
        skos:Concept ,
        surv:SurveyPurpose ;
    skos:definition "To depict a subsidiary proposed Unit Development CSD produced under the Unit Titles Act 2010. No survey system information is provided. Tenure system information may be used, or adopted for use, in defining applicable interests in unit tenures." ;
    skos:inScheme cs: ;
    skos:notation "spud" ;
    skos:prefLabel "Subsidiary Proposed Unit Development" ;
    skos:topConceptOf cs: ;
.

:spud-ss
    a
        skos:Concept ,
        surv:SurveyPurpose ;
    skos:definition "To depict a subsidiary proposed Unit Development CSD with survey sheet, produced under the Unit Titles Act 2010. Survey system information may be adopted by other surveys. Tenure system information may be used to define interests in units, easements or covenants only." ;
    skos:inScheme cs: ;
    skos:notation "spud-ss" ;
    skos:prefLabel "Subsidiary Proposed Unit Development with Survey Sheet" ;
    skos:topConceptOf cs: ;
.

:srup
    a
        skos:Concept ,
        surv:SurveyPurpose ;
    skos:definition "To depict a simple redevelopment Unit Title CSD produced under the Unit Titles Act 2010. No survey system information is provided. Tenure system information may be used, or adopted for use, in defining applicable interests in unit tenures." ;
    skos:inScheme cs: ;
    skos:notation "srup" ;
    skos:prefLabel "Simple Redevelopment Unit Plan" ;
    skos:topConceptOf cs: ;
.

:srup-ss
    a
        skos:Concept ,
        surv:SurveyPurpose ;
    skos:definition "To depict a simple redevelopment Unit Title CSD with survey sheet produced under the Unit Titles Act 2010. Survey system information may be adopted by other surveys. Tenure system information may be used to define interests in units, easements or covenants only." ;
    skos:inScheme cs: ;
    skos:notation "srup-ss" ;
    skos:prefLabel "Simple Redevelopment Unit Plan with Survey Sheet" ;
    skos:topConceptOf cs: ;
.

:ssup
    a
        skos:Concept ,
        surv:SurveyPurpose ;
    skos:definition "To depict a subsidiary standard Unit Title CSD produced under the Unit Titles Act 2010. No survey system information is provided. Tenure system information may be used, or adopted for use, in defining applicable interests in unit tenures." ;
    skos:inScheme cs: ;
    skos:notation "ssup" ;
    skos:prefLabel "Subsidiary Standard Unit Plan" ;
    skos:topConceptOf cs: ;
.

:ssup-ss
    a
        skos:Concept ,
        surv:SurveyPurpose ;
    skos:definition "To depict a subsidiary standard Unit Title CSD with survey sheet produced under the Unit Titles Act 2010. Survey system information may be adopted by other surveys. Tenure system information may be used to define interests in units, easements or covenants only." ;
    skos:inScheme cs: ;
    skos:notation "ssup-ss" ;
    skos:prefLabel "Subsidiary Standard Unit Plan with Survey Sheet" ;
    skos:topConceptOf cs: ;
.

:stage-up
    a
        skos:Concept ,
        surv:SurveyPurpose ;
    skos:definition "To depict a further stage (other than the complete stage) of a Unit Title staged development CSD produced under the Unit Titles Act 1972 and the Unit Titles Amendment Act 1979. No survey system information is provided. Tenure system information may be used, or adopted for use, in defining applicable interests in unit tenures." ;
    skos:inScheme cs: ;
    skos:notation "stage-up" ;
    skos:prefLabel "Stage Unit Plan" ;
    skos:topConceptOf cs: ;
.

:stage-up-ss
    a
        skos:Concept ,
        surv:SurveyPurpose ;
    skos:definition "To depict a further stage (other than the complete stage) of a Unit Title staged development CSD with survey sheet, produced under the Unit Titles Act 1972 and the Unit Titles Amendment Act 1979. Survey system information may be adopted by other surveys. Tenure system information may be used to define interests in units, easements or covenants only." ;
    skos:inScheme cs: ;
    skos:notation "stage-up-ss" ;
    skos:prefLabel "Stage Unit Plan with Survey Sheet" ;
    skos:topConceptOf cs: ;
.

:sub-pud
    a
        skos:Concept ,
        surv:SurveyPurpose ;
    skos:definition "To depict a substituted proposed Unit Title staged development CSD produced under the Unit Titles Act 1972 and the Unit Titles Amendment Act 1979. No survey system information is provided. Tenure system information may be used, or adopted for use, in defining applicable interests in unit tenures." ;
    skos:inScheme cs: ;
    skos:notation "sub-pud" ;
    skos:prefLabel "Substituted Proposed Unit Development" ;
    skos:topConceptOf cs: ;
.

:sub-udp-ss
    a
        skos:Concept ,
        surv:SurveyPurpose ;
    skos:definition "To depict a substituted proposed Unit Title staged development CSD with survey sheet produced under the Unit Titles Act 1972 and the Unit Titles Amendment Act 1979. Survey system information may be adopted by other surveys. Tenure system information may be used to define interests in units, easements or covenants only." ;
    skos:inScheme cs: ;
    skos:notation "sub-udp-ss" ;
    skos:prefLabel "Substituted Proposed Unit Development with Survey Sheet" ;
    skos:topConceptOf cs: ;
.

:sup
    a
        skos:Concept ,
        surv:SurveyPurpose ;
    skos:definition "To depict a standard Unit Title CSD produced under the Unit Titles Act 1972. No survey system information is provided. Tenure system information may be used, or adopted for use, in defining applicable interests in unit tenures." ;
    skos:inScheme cs: ;
    skos:notation "sup" ;
    skos:prefLabel "Standard Unit Plan" ;
    skos:topConceptOf cs: ;
.

:sup-ss
    a
        skos:Concept ,
        surv:SurveyPurpose ;
    skos:definition "To depict a standard Unit Title CSD with survey sheet produced under the Unit Titles Act 1972. Survey system information may be adopted by other surveys. Tenure system information may be used to define interests in units, easements or covenants only." ;
    skos:inScheme cs: ;
    skos:notation "sup-ss" ;
    skos:prefLabel "Standard Unit Plan with Survey Sheet" ;
    skos:topConceptOf cs: ;
.

:sv
    a
        skos:Concept ,
        surv:SurveyPurpose ;
    skos:definition "To depict the boundary of a land area when such is required for Statutory vesting purposes only. Survey system information may be adopted by other surveys. Tenure system information to be used for the Statutory vesting purposes only. It is NOT to be used for any land tenure or title purposes." ;
    skos:inScheme cs: ;
    skos:notation "sv" ;
    skos:prefLabel "Statutory Vesting" ;
    skos:topConceptOf cs: ;
.

:ups
    a
        skos:Concept ,
        surv:SurveyPurpose ;
    skos:definition "To depict a standard Unit Title ‘CSD in substitution’ produced under the Unit Titles Act 1972. No survey system information is provided. Tenure system information may be used, or adopted for use, in defining applicable interests in unit tenures." ;
    skos:inScheme cs: ;
    skos:notation "ups" ;
    skos:prefLabel "Unit Plan in Substitution" ;
    skos:topConceptOf cs: ;
.

:ups-ss
    a
        skos:Concept ,
        surv:SurveyPurpose ;
    skos:definition "To depict Unit Title ‘CSD in substitution’ with survey sheet produced under the Unit Titles Act 1972. Survey system information  may be adopted by other surveys. Tenure system information may be used to define interests in units, easements or covenants only." ;
    skos:inScheme cs: ;
    skos:notation "ups-ss" ;
    skos:prefLabel "Unit Plan in Substitution with Survey Sheet" ;
    skos:topConceptOf cs: ;
.

<https://linked.data.gov.au/org/csdm-pg>
    a schema:Organization ;
    schema:name "CSDM Project Group" ;
    schema:parentOrganization <https://linked.data.gov.au/org/icsm> ;
    schema:url "https://icsm-au.github.io/3d-csdm/docs/"^^xsd:anyURI ;
.

<https://linked.data.gov.au/org/icsm>
    a schema:Organization ;
    schema:name "Intergovernmental Committee on Surveying & Mapping" ;
    schema:url "https://icsm.gov.au"^^xsd:anyURI ;
.

cs:
    a skos:ConceptScheme ;
    skos:definition "NZ Survey Purpose"@en ;
    skos:hasTopConcept
        :amalgamation ,
        :application ,
        :cbr ,
        :ce ,
        :cfl ,
        :consolidation ,
        :csp ,
        :csup ,
        :csup-ss ,
        :easement ,
        :fpcp ,
        :fpcp-ss ,
        :fsup ,
        :fsup-ss ,
        :h-c-s ,
        :h-cbr ,
        :h-covenant ,
        :h-na ,
        :h-s-i ,
        :h-sbr ,
        :lease ,
        :legalisation ,
        :lt ,
        :ltlc ,
        :lts ,
        :mf ,
        :mining ,
        :n-c ,
        :partition ,
        :pud ,
        :pud-ss ,
        :reclamation ,
        :revesting ,
        :roadway ,
        :rup ,
        :rup-ss ,
        :sbr ,
        :se-r ,
        :si ,
        :soplc ,
        :spud ,
        :spud-ss ,
        :srup ,
        :srup-ss ,
        :ssup ,
        :ssup-ss ,
        :stage-up ,
        :stage-up-ss ,
        :sub-pud ,
        :sub-udp-ss ,
        :sup ,
        :sup-ss ,
        :sv ,
        :ups ,
        :ups-ss ;
    skos:prefLabel "NZ Survey Purpose" ;
    skos:scopeNote "surv:SurveyPurpose" ;
    schema:creator <https://linked.data.gov.au/org/csdm-pg> ;
    schema:dateCreated "2022-03-18"^^xsd:date ;
    schema:dateModified "2024-08-20"^^xsd:date ;
    schema:keywords unggim:LandParcels ;
    schema:publisher <https://linked.data.gov.au/org/icsm> ;
.

[]    a prov:Activity ;
    prov:endedAtTime "2024-04-11T06:11:42.742287"^^xsd:dateTime ;
    prov:startedAtTime "2024-04-11T06:11:42.629933"^^xsd:dateTime ;
    prov:used
        [
            a prov:Entity ;
            dct:format "application/json" ;
            dct:hasVersion "git:29bbdd91c50914400e0758872364ec1cea2d1501" ;
            rdfs:seeAlso "file:///home/runner/work/icsm-vocabs/icsm-vocabs/cadastre/CSD-Header/nz-survey-purpose.csv" ;
        ] ;
    prov:wasAssociatedWith
        [
            a
                prov:Agent ,
                schema:SoftwareApplication ;
            rdfs:label "OGC-NA tools" ;
            dct:hasVersion "0.3.44" ;
            rdfs:seeAlso "https://github.com/opengeospatial/ogc-na-tools" ;
        ] ;
    prov:wasInformedBy
        [
            dct:identifier "42611fe7-ad51-40e1-adf8-e3a0f1ee7a83" ;
        ] ; ;
.
