PREFIX : <https://linked.data.gov.au/def/csdm/nz-survey-class/>
PREFIX cs: <https://linked.data.gov.au/def/csdm/nz-survey-class>
PREFIX dct: <http://purl.org/dc/terms/>
PREFIX prov: <http://www.w3.org/ns/prov#>
PREFIX rdfs: <http://www.w3.org/2000/01/rdf-schema#>
PREFIX schema: <https://schema.org/>
PREFIX skos: <http://www.w3.org/2004/02/skos/core#>
PREFIX termtype: <https://linked.data.gov.au/def/csdm/termtypes/>
PREFIX unggim: <https://linked.data.gov.au/def/unggim-themes/>
PREFIX xsd: <http://www.w3.org/2001/XMLSchema#>

:a
    a
        skos:Concept ,
        termtype:SurveyType ;
    skos:definition "Urban and the most accurate. The class A tolerance for boundary points increases from 0.06m at a rate of 0.015m per 100m." ;
    skos:inScheme cs: ;
    skos:notation "a" ;
    skos:prefLabel "Class A" ;
    skos:topConceptOf cs: ;
.

:b
    a
        skos:Concept ,
        termtype:SurveyType ;
    skos:definition "Rural and not as accurate as class A. The class B tolerance for boundary points increases from 0.30m at a rate of 0.06m per 100m." ;
    skos:inScheme cs: ;
    skos:notation "b" ;
    skos:prefLabel "Class B" ;
    skos:topConceptOf cs: ;
.

:c
    a
        skos:Concept ,
        termtype:SurveyType ;
    skos:definition "Used in specified rural circumstances where a less accurate boundary is acceptable. The class C tolerance for boundary points increases from 1.00m at a rate of 0.30m per 100m." ;
    skos:inScheme cs: ;
    skos:notation "c" ;
    skos:prefLabel "Class C" ;
    skos:topConceptOf cs: ;
.

:d
    a
        skos:Concept ,
        termtype:SurveyType ;
    skos:definition "(used in exceptional circumstances where the existing boundary accuracy is unknown or unable to be determined and it is appropriate to permit these inaccuracies to remain" ;
    skos:inScheme cs: ;
    skos:notation "d" ;
    skos:prefLabel "Class D" ;
    skos:topConceptOf cs: ;
.

<https://linked.data.gov.au/org/csdm-pg>
    a schema:Organization ;
    schema:name "CSDM Project Group" ;
    schema:parentOrganization <https://linked.data.gov.au/org/icsm> ;
    schema:url "https://icsm-au.github.io/3d-csdm/docs/"^^xsd:anyURI ;
.

<https://linked.data.gov.au/org/icsm>
    a schema:Organization ;
    schema:name "Intergovernmental Committee on Surveying & Mapping" ;
    schema:url "https://icsm.gov.au"^^xsd:anyURI ;
.

cs:
    a skos:ConceptScheme ;
    skos:definition "NZ Survey Class"@en ;
    skos:hasTopConcept
        :a ,
        :b ,
        :c ,
        :d ;
    skos:prefLabel "NZ Survey Class" ;
    skos:scopeNote "termtype:SurveyType" ;
    schema:creator <https://linked.data.gov.au/org/csdm-pg> ;
    schema:dateCreated "2022-03-18"^^xsd:date ;
    schema:dateModified "2024-08-20"^^xsd:date ;
    schema:keywords unggim:LandParcels ;
    schema:publisher <https://linked.data.gov.au/org/icsm> ;
.

[]    a prov:Activity ;
    prov:endedAtTime "2024-04-11T06:11:35.723434"^^xsd:dateTime ;
    prov:startedAtTime "2024-04-11T06:11:35.630600"^^xsd:dateTime ;
    prov:used
        [
            a prov:Entity ;
            dct:format "application/json" ;
            dct:hasVersion "git:29bbdd91c50914400e0758872364ec1cea2d1501" ;
            rdfs:seeAlso "file:///home/runner/work/icsm-vocabs/icsm-vocabs/cadastre/CSD-Header/nz-survey-class.csv" ;
        ] ;
    prov:wasAssociatedWith
        [
            a
                prov:Agent ,
                schema:SoftwareApplication ;
            rdfs:label "OGC-NA tools" ;
            dct:hasVersion "0.3.44" ;
            rdfs:seeAlso "https://github.com/opengeospatial/ogc-na-tools" ;
        ] ;
    prov:wasInformedBy
        [
            dct:identifier "42611fe7-ad51-40e1-adf8-e3a0f1ee7a83" ;
        ] ; ;
.
