PREFIX : <https://linked.data.gov.au/def/csdm/nz-survey-documentation-type/>
PREFIX cs: <https://linked.data.gov.au/def/csdm/nz-survey-documentation-type>
PREFIX dcterms: <http://purl.org/dc/terms/>
PREFIX prov: <http://www.w3.org/ns/prov#>
PREFIX rdfs: <http://www.w3.org/2000/01/rdf-schema#>
PREFIX schema: <https://schema.org/>
PREFIX skos: <http://www.w3.org/2004/02/skos/core#>
PREFIX termtype: <https://linked.data.gov.au/def/csdm/termtypes/>
PREFIX unggim: <https://linked.data.gov.au/def/unggim-themes/>
PREFIX xsd: <http://www.w3.org/2001/XMLSchema#>

:a-rqt
    a
        skos:Concept ,
        termtype:DocType ;
    skos:definition "Request from a surveyor giving authority for a change to be made to their survey." ;
    skos:inScheme cs: ;
    skos:notation "a-rqt" ;
    skos:prefLabel "Amendments Request" ;
    skos:topConceptOf cs: ;
.

:aca
    a
        skos:Concept ,
        termtype:DocType ;
    skos:definition "Affidavit required in support of the claim for accretion to land. Declaration by an independent person verifying that accretion has been caused by the slow and imperceptible build up of land." ;
    skos:inScheme cs: ;
    skos:notation "aca" ;
    skos:prefLabel "Accretion Claim Affidavit" ;
    skos:topConceptOf cs: ;
.

:acpi
    a
        skos:Concept ,
        termtype:DocType ;
    skos:definition "Additional image of a colour plan." ;
    skos:inScheme cs: ;
    skos:notation "acpi" ;
    skos:prefLabel "Additional Colour Plan Image" ;
    skos:topConceptOf cs: ;
.

:af
    a
        skos:Concept ,
        termtype:DocType ;
    skos:definition "Form approved for use in registration, either by the Registrar General of Land (RGL) or Senior Regulatory Adviser (SRA). Any fees are paid against the instrument type FAP." ;
    skos:inScheme cs: ;
    skos:notation "af" ;
    skos:prefLabel "Approved Form" ;
    skos:topConceptOf cs: ;
.

:al
    a
        skos:Concept ,
        termtype:DocType ;
    skos:definition "List of amendments required to amend a cadastral survey transaction." ;
    skos:inScheme cs: ;
    skos:notation "al" ;
    skos:prefLabel "Amendment List" ;
    skos:topConceptOf cs: ;
.

:andm
    a
        skos:Concept ,
        termtype:DocType ;
    skos:definition "Correspondence that may accompany a plan returned from the Maori Land Court with the Judge's signature." ;
    skos:inScheme cs: ;
    skos:notation "andm" ;
    skos:prefLabel "Approved notice from MLC" ;
    skos:topConceptOf cs: ;
.

:aod
    a
        skos:Concept ,
        termtype:DocType ;
    skos:definition "Adjoining owners consents for the definition of boundaries as set out in the survey." ;
    skos:inScheme cs: ;
    skos:notation "aod" ;
    skos:prefLabel "Adjoining Owners Declarations" ;
    skos:topConceptOf cs: ;
.

:ar
    a
        skos:Concept ,
        termtype:DocType ;
    skos:definition "Report of the items amended for a cadastral survey transaction and how the amendments were done." ;
    skos:inScheme cs: ;
    skos:notation "ar" ;
    skos:prefLabel "Amendment Report" ;
    skos:topConceptOf cs: ;
.

:ard
    a
        skos:Concept ,
        termtype:DocType ;
    skos:definition "Declined request for issue of an appellation for the creation of a parcel of land." ;
    skos:inScheme cs: ;
    skos:notation "ard" ;
    skos:prefLabel "Appellation Request Declined" ;
    skos:topConceptOf cs: ;
.

:as
    a
        skos:Concept ,
        termtype:DocType ;
    skos:definition "Schedule of parcels defined in an e-survey for Legalisation or Crown Subdivision purposes. Contains information such as legal description, land status and proposed action. Not to be used for easement/covenant information or for Land Transfer Plans. This SUD type does not bundle with the CSD or Title Plans." ;
    skos:inScheme cs: ;
    skos:notation "as" ;
    skos:prefLabel "Area Schedule" ;
    skos:topConceptOf cs: ;
.

:c
    a
        skos:Concept ,
        termtype:DocType ;
    skos:definition "Letters and other correspondence associated with the survey." ;
    skos:inScheme cs: ;
    skos:notation "c" ;
    skos:prefLabel "Correspondence" ;
    skos:topConceptOf cs: ;
.

:c-p
    a
        skos:Concept ,
        termtype:DocType ;
    skos:definition "Miscellaneous consents. Note consents to the deposit of unit plans have a document type of CON and fees are recorded against that instrument type." ;
    skos:inScheme cs: ;
    skos:notation "c-p" ;
    skos:prefLabel "Consent / Permit" ;
    skos:topConceptOf cs: ;
.

:c-t
    a
        skos:Concept ,
        termtype:DocType ;
    skos:definition "Trustee details for Friendly Societies, etc (as opposed to Charitable Trusts). No fees are paid and the application is not registered." ;
    skos:inScheme cs: ;
    skos:notation "c-t" ;
    skos:prefLabel "Change of Trustee" ;
    skos:topConceptOf cs: ;
.

:co
    a
        skos:Concept ,
        termtype:DocType ;
    skos:definition "Court Orders received for Lapsing of Caveats, Joint Family Home advertising etc." ;
    skos:inScheme cs: ;
    skos:notation "co" ;
    skos:prefLabel "Court Order" ;
    skos:topConceptOf cs: ;
.

:cs
    a
        skos:Concept ,
        termtype:DocType ;
    skos:definition "Sheet of calculations associated with the survey." ;
    skos:inScheme cs: ;
    skos:notation "cs" ;
    skos:prefLabel "Calculation Sheet" ;
    skos:topConceptOf cs: ;
.

:cslb-d
    a
        skos:Concept ,
        termtype:DocType ;
    skos:definition "A Supervision Order requested by the Cadastral Survey Licensing Board (CSLB). The affected surveyor submits their survey with a letter from another licensed surveyor (attached as a supporting document) stating that the survey meets the survey rule requirements. The CSLB will advise the affected surveyor when this supporting document type is to be used." ;
    skos:inScheme cs: ;
    skos:notation "cslb-d" ;
    skos:prefLabel "CSLB (Cadastral Survey Licensing Board) Document" ;
    skos:topConceptOf cs: ;
.

:cspt-dlr
    a
        skos:Concept ,
        termtype:DocType ;
    skos:definition "A report prepared by the approving surveyor outlining any anomalies found by a cadastral survey with existing title." ;
    skos:inScheme cs: ;
    skos:notation "cspt-dlr" ;
    skos:prefLabel "Chief Surveyors Plan Report to DLR" ;
    skos:topConceptOf cs: ;
.

:d-doc
    a
        skos:Concept ,
        termtype:DocType ;
    skos:definition "Document deposited to support a survey." ;
    skos:inScheme cs: ;
    skos:notation "d-doc" ;
    skos:prefLabel "Deposit Document" ;
    skos:topConceptOf cs: ;
.

:dar
    a
        skos:Concept ,
        termtype:DocType ;
    skos:definition "Report details from Chief Surveyor recommending disciplinary action against a Surveyor." ;
    skos:inScheme cs: ;
    skos:notation "dar" ;
    skos:prefLabel "Disciplinary Action Recommendation" ;
    skos:topConceptOf cs: ;
.

:db-mlc
    a
        skos:Concept ,
        termtype:DocType ;
    skos:definition "Description of the land as set out by the MLC. Māori Land Court Order copy associated with a Māori Land survey." ;
    skos:inScheme cs: ;
    skos:notation "db-mlc" ;
    skos:prefLabel "Description of Boundaries ML Court" ;
    skos:topConceptOf cs: ;
.

:dd
    a
        skos:Concept ,
        termtype:DocType ;
    skos:definition "Details of a particular datum used for a survey." ;
    skos:inScheme cs: ;
    skos:notation "dd" ;
    skos:prefLabel "Datum Details" ;
    skos:topConceptOf cs: ;
.

:dlpf
    a
        skos:Concept ,
        termtype:DocType ;
    skos:definition "A template form for the surveyor to complete to indicate the complexity of the e-survey." ;
    skos:inScheme cs: ;
    skos:notation "dlpf" ;
    skos:prefLabel "Dataset Lodgement Profile Form" ;
    skos:topConceptOf cs: ;
.

:edd
    a
        skos:Concept ,
        termtype:DocType ;
    skos:definition "A request accompanying a manual dealing requesting LINZ to exempt the conveyancer from having to present it as an e-dealing." ;
    skos:inScheme cs: ;
    skos:notation "edd" ;
    skos:prefLabel "E-Dealing Dispensation" ;
    skos:topConceptOf cs: ;
.

:eir
    a
        skos:Concept ,
        termtype:DocType ;
    skos:definition "Report detailing the errors identified and the impact on other data." ;
    skos:inScheme cs: ;
    skos:notation "eir" ;
    skos:prefLabel "Error Item Report" ;
    skos:topConceptOf cs: ;
.

:esftpr
    a
        skos:Concept ,
        termtype:DocType ;
    skos:definition "Requests priority processing for an e-survey with an associated lodged dealing. This document is available as a .pdf on the LINZ website. Solicitors can lodge an e-request via workspace, which is automated." ;
    skos:inScheme cs: ;
    skos:notation "esftpr" ;
    skos:prefLabel "E-Survey Fast Track Processing Request Form" ;
    skos:topConceptOf cs: ;
.

:et
    a
        skos:Concept ,
        termtype:DocType ;
    skos:definition "Report of equipment test results." ;
    skos:inScheme cs: ;
    skos:notation "et" ;
    skos:prefLabel "Equipment Test" ;
    skos:topConceptOf cs: ;
.

:f-r
    a
        skos:Concept ,
        termtype:DocType ;
    skos:definition "Instructions issued for field audit of a cadastral survey." ;
    skos:inScheme cs: ;
    skos:notation "f-r" ;
    skos:prefLabel "Field Request" ;
    skos:topConceptOf cs: ;
.

:fi
    a
        skos:Concept ,
        termtype:DocType ;
    skos:definition "Record of observations taken in the field by a surveyor and associated with the survey." ;
    skos:inScheme cs: ;
    skos:notation "fi" ;
    skos:prefLabel "Field Information" ;
    skos:topConceptOf cs: ;
.

:fq
    a
        skos:Concept ,
        termtype:DocType ;
    skos:definition "A fee query linked to an associated e-dealing or e-survey." ;
    skos:inScheme cs: ;
    skos:notation "fq" ;
    skos:prefLabel "Fee Query" ;
    skos:topConceptOf cs: ;
.

:fr
    a
        skos:Concept ,
        termtype:DocType ;
    skos:definition "The report prepared after field audit of a survey." ;
    skos:inScheme cs: ;
    skos:notation "fr" ;
    skos:prefLabel "Field Report" ;
    skos:topConceptOf cs: ;
.

:go
    a
        skos:Concept ,
        termtype:DocType ;
    skos:definition "Miscellaneous geodetic report associated with a geodetic work." ;
    skos:inScheme cs: ;
    skos:notation "go" ;
    skos:prefLabel "Geodetic Other" ;
    skos:topConceptOf cs: ;
.

:gwr
    a
        skos:Concept ,
        termtype:DocType ;
    skos:definition "A report supplied by a geodetic contractor giving details of a geodetic work." ;
    skos:inScheme cs: ;
    skos:notation "gwr" ;
    skos:prefLabel "Geodetic Work Report" ;
    skos:topConceptOf cs: ;
.

:lf
    a
        skos:Concept ,
        termtype:DocType ;
    skos:definition "A form included with a survey or dealing transaction when manually lodged." ;
    skos:inScheme cs: ;
    skos:notation "lf" ;
    skos:prefLabel "Lodgement Form" ;
    skos:topConceptOf cs: ;
.

:m
    a
        skos:Concept ,
        termtype:DocType ;
    skos:definition "Memoranda under s209 Land Transfer Act 2017 (also registered as a document)." ;
    skos:inScheme cs: ;
    skos:notation "m" ;
    skos:prefLabel "Memorandum" ;
    skos:topConceptOf cs: ;
.

:m-vr
    a
        skos:Concept ,
        termtype:DocType ;
    skos:definition "Mark and Vectors report for the e-survey." ;
    skos:inScheme cs: ;
    skos:notation "m-vr" ;
    skos:prefLabel "Mark and Vectors Report" ;
    skos:topConceptOf cs: ;
.

:md
    a
        skos:Concept ,
        termtype:DocType ;
    skos:definition "Details of a survey mark. Usually associated with a geodetic mark." ;
    skos:inScheme cs: ;
    skos:notation "md" ;
    skos:prefLabel "Mark Details" ;
    skos:topConceptOf cs: ;
.

:mp
    a
        skos:Concept ,
        termtype:DocType ;
    skos:definition "Photograph of a mark. Usually associated with a geodetic mark." ;
    skos:inScheme cs: ;
    skos:notation "mp" ;
    skos:prefLabel "Mark Photograph" ;
    skos:topConceptOf cs: ;
.

:nc
    a
        skos:Concept ,
        termtype:DocType ;
    skos:definition "Confirmation of location of a proposed node/mark." ;
    skos:inScheme cs: ;
    skos:notation "nc" ;
    skos:prefLabel "Node Confirmation" ;
    skos:topConceptOf cs: ;
.

:o-r
    a
        skos:Concept ,
        termtype:DocType ;
    skos:definition "The instructions issued for an office audit of a cadastral survey." ;
    skos:inScheme cs: ;
    skos:notation "o-r" ;
    skos:prefLabel "Office Request" ;
    skos:topConceptOf cs: ;
.

:oc
    a
        skos:Concept ,
        termtype:DocType ;
    skos:definition "Owner's consent or  adjoining owner's consent submitted as a separate document but as part of a transaction." ;
    skos:inScheme cs: ;
    skos:notation "oc" ;
    skos:prefLabel "Owners Consent" ;
    skos:topConceptOf cs: ;
.

:od
    a
        skos:Concept ,
        termtype:DocType ;
    skos:definition "Diagram of occupation associated with the survey to attach to a Digital Survey Plan." ;
    skos:inScheme cs: ;
    skos:notation "od" ;
    skos:prefLabel "Occupation Diagram" ;
    skos:topConceptOf cs: ;
.

:or
    a
        skos:Concept ,
        termtype:DocType ;
    skos:definition "Report prepared after office audit of a cadastral survey." ;
    skos:inScheme cs: ;
    skos:notation "or" ;
    skos:prefLabel "Office Report" ;
    skos:topConceptOf cs: ;
.

:p-ar
    a
        skos:Concept ,
        termtype:DocType ;
    skos:definition "A request for LINZ to allocate one or more new title numbers what will issue when a land transfer survey deposits." ;
    skos:inScheme cs: ;
    skos:notation "p-ar" ;
    skos:prefLabel "Pre-Allocation Request" ;
    skos:topConceptOf cs: ;
.

:p-crl
    a
        skos:Concept ,
        termtype:DocType ;
    skos:definition "A copy of a rejection letter or report from LINZ attached to the re-lodged dealing or survey." ;
    skos:inScheme cs: ;
    skos:notation "p-crl" ;
    skos:prefLabel "Pre-Check Rejection Letter" ;
    skos:topConceptOf cs: ;
.

:p-d
    a
        skos:Concept ,
        termtype:DocType ;
    skos:definition "Plot or diagram to support survey definition, e.g., aerial photograph, digitised stream fix." ;
    skos:inScheme cs: ;
    skos:notation "p-d" ;
    skos:prefLabel "Plot / Diagram" ;
    skos:topConceptOf cs: ;
.

:pa
    a
        skos:Concept ,
        termtype:DocType ;
    skos:definition "Power of Attorney summary (also registered as a document)." ;
    skos:inScheme cs: ;
    skos:notation "pa" ;
    skos:prefLabel "Power of Attorney" ;
    skos:topConceptOf cs: ;
.

:pg
    a
        skos:Concept ,
        termtype:DocType ;
    skos:definition "Commonly used to depict parcels on CSD's that have permanent structure boundaries or stratum boundaries, e.g., Unit & Cross Lease CSD's. Can be used to show plan, elevation or cross-section views. The Plan Graphic forms part of the Survey Diagram and Diagram of Parcels and bundles with the CSD and Title Plans. This SUD type can also be used for a plan returned from the Maori Land Court signed by the Judge to attach to CSD and Title Plans." ;
    skos:inScheme cs: ;
    skos:notation "pg" ;
    skos:prefLabel "Plan Graphic" ;
    skos:topConceptOf cs: ;
.

:psbg
    a
        skos:Concept ,
        termtype:DocType ;
    skos:definition "Used to depict easements defined by Permanent Structure Boundaries where survey purpose is Easement, Lease or Statutory Easement/Right.  When this supporting document type is selected, the attached documents are incorporated into the CSD or Title Plan images, allowing the CSD to be submitted without spatial capture." ;
    skos:inScheme cs: ;
    skos:notation "psbg" ;
    skos:prefLabel "PSB Non Primary Graphic (PSBG)" ;
    skos:topConceptOf cs: ;
.

:r-rr
    a
        skos:Concept ,
        termtype:DocType ;
    skos:definition "An online form provided by LINZ to allow conveyancers and surveyors to request LINZ to review the reasons for rejection or requisition of a dealing or survey." ;
    skos:inScheme cs: ;
    skos:notation "r-rr" ;
    skos:prefLabel "Requisition/Rejection Review" ;
    skos:topConceptOf cs: ;
.

:r-sfr
    a
        skos:Concept ,
        termtype:DocType ;
    skos:definition "An online form provided by LINZ to allow conveyancers and surveyors to request LINZ to review the fees for rejection or requisition of a dealing or survey." ;
    skos:inScheme cs: ;
    skos:notation "r-sfr" ;
    skos:prefLabel "Re-submission Fee Review" ;
    skos:topConceptOf cs: ;
.

:rrn
    a
        skos:Concept ,
        termtype:DocType ;
    skos:definition "Surveyors reply to a requisition associated with a survey." ;
    skos:inScheme cs: ;
    skos:notation "rrn" ;
    skos:prefLabel "Response to Requisition Notice" ;
    skos:topConceptOf cs: ;
.

:s-m
    a
        skos:Concept ,
        termtype:DocType ;
    skos:definition "Schedule or memorandum containing information about easements as required by Rule 10.2 of the Rules for Cadastral Survey 2010. Can also be used for recording covenant information required by Rule 10.3 of the Rules for Cadastral Survey 2010." ;
    skos:inScheme cs: ;
    skos:notation "s-m" ;
    skos:prefLabel "Schedule / Memorandum" ;
    skos:topConceptOf cs: ;
.

:s211
    a
        skos:Concept ,
        termtype:DocType ;
    skos:definition "Request by the Senior Regulatory Adviser (SRA) for a customer to produce an instrument or title." ;
    skos:inScheme cs: ;
    skos:notation "s211" ;
    skos:prefLabel "Request to produce instrument (s211 Land Transfer Act 1952)" ;
    skos:topConceptOf cs: ;
.

:sar
    a
        skos:Concept ,
        termtype:DocType ;
    skos:definition "A report by a surveyor as required by Rule 8.2 of the Rules for Cadastral Survey 2010." ;
    skos:inScheme cs: ;
    skos:notation "sar" ;
    skos:prefLabel "Survey Assistance Report" ;
    skos:topConceptOf cs: ;
.

:schp
    a
        skos:Concept ,
        termtype:DocType ;
    skos:definition "Geodetic network planning." ;
    skos:inScheme cs: ;
    skos:notation "schp" ;
    skos:prefLabel "Scheme Plan" ;
    skos:topConceptOf cs: ;
.

:sd
    a
        skos:Concept ,
        termtype:DocType ;
    skos:definition "Details of a geodetic site which may contain one or more survey marks." ;
    skos:inScheme cs: ;
    skos:notation "sd" ;
    skos:prefLabel "Site Details" ;
    skos:topConceptOf cs: ;
.

:sdg
    a
        skos:Concept ,
        termtype:DocType ;
    skos:definition "A type of plan graphic containing survey data to be incorporated with the Record of Survey. Used to depict survey data that is not required to be captured by the Standard for lodgement of cadastral survey datasets (LINZS70000). For example can be used for recording survey data on Simple and Complex Boundary Reinstatement CSDs." ;
    skos:inScheme cs: ;
    skos:notation "sdg" ;
    skos:prefLabel "Survey Data Graphic" ;
    skos:topConceptOf cs: ;
.

:sfw
    a
        skos:Concept ,
        termtype:DocType ;
    skos:definition "Report associated with searching." ;
    skos:inScheme cs: ;
    skos:notation "sfw" ;
    skos:prefLabel "Search Fee Wastage" ;
    skos:topConceptOf cs: ;
.

:sp
    a
        skos:Concept ,
        termtype:DocType ;
    skos:definition "Photo of survey monuments (usually associated with geodetic marks)." ;
    skos:inScheme cs: ;
    skos:notation "sp" ;
    skos:prefLabel "Site Photograph" ;
    skos:topConceptOf cs: ;
.

:sr
    a
        skos:Concept ,
        termtype:DocType ;
    skos:definition "A report by a surveyor giving details of a survey as required under the Surveyor-Generals Guidelines." ;
    skos:inScheme cs: ;
    skos:notation "sr" ;
    skos:prefLabel "Survey Report" ;
    skos:topConceptOf cs: ;
.

:ta-c
    a
        skos:Concept ,
        termtype:DocType ;
    skos:definition "Certification from a TA to attach to a Digital Survey Plan and Digital Title Plan." ;
    skos:inScheme cs: ;
    skos:notation "ta-c" ;
    skos:prefLabel "Territorial Authority (TA) Certificate" ;
    skos:topConceptOf cs: ;
.

:tac
    a
        skos:Concept ,
        termtype:DocType ;
    skos:definition "Miscellaneous.  Territorial Authority correspondence associated with the survey." ;
    skos:inScheme cs: ;
    skos:notation "tac" ;
    skos:prefLabel "TA Correspondence" ;
    skos:topConceptOf cs: ;
.

:tacpi
    a
        skos:Concept ,
        termtype:DocType ;
    skos:definition "A scanned image of a certified paper survey plan." ;
    skos:inScheme cs: ;
    skos:notation "tacpi" ;
    skos:prefLabel "Territorial Authority (TA) Certificate  Plan Image" ;
    skos:topConceptOf cs: ;
.

:ts
    a
        skos:Concept ,
        termtype:DocType ;
    skos:definition "Traverse sheets associated with the survey." ;
    skos:inScheme cs: ;
    skos:notation "ts" ;
    skos:prefLabel "Traverse Sheet" ;
    skos:topConceptOf cs: ;
.

:uevc
    a
        skos:Concept ,
        termtype:DocType ;
    skos:definition "Valuer's Unit Entitlement and Certification for Unit Developments." ;
    skos:inScheme cs: ;
    skos:notation "uevc" ;
    skos:prefLabel "Unit Entitlements and Valuers Certification" ;
    skos:topConceptOf cs: ;
.

:wbr
    a
        skos:Concept ,
        termtype:DocType ;
    skos:definition "Record of the position of any new water boundary associated with the survey." ;
    skos:inScheme cs: ;
    skos:notation "wbr" ;
    skos:prefLabel "Water Boundary Record" ;
    skos:topConceptOf cs: ;
.

:wi-d
    a
        skos:Concept ,
        termtype:DocType ;
    skos:definition "Request to withdraw an instrument or dealing." ;
    skos:inScheme cs: ;
    skos:notation "wi-d" ;
    skos:prefLabel "Withdraw Instrument/Dealing" ;
    skos:topConceptOf cs: ;
.

cs:
    a skos:ConceptScheme ;
    skos:definition "NZ types of Survey Documentation"@en ;
    skos:hasTopConcept
        :a-rqt ,
        :aca ,
        :acpi ,
        :af ,
        :al ,
        :andm ,
        :aod ,
        :ar ,
        :ard ,
        :as ,
        :c ,
        :c-p ,
        :c-t ,
        :co ,
        :cs ,
        :cslb-d ,
        :cspt-dlr ,
        :d-doc ,
        :dar ,
        :db-mlc ,
        :dd ,
        :dlpf ,
        :edd ,
        :eir ,
        :esftpr ,
        :et ,
        :f-r ,
        :fi ,
        :fq ,
        :fr ,
        :go ,
        :gwr ,
        :lf ,
        :m ,
        :m-vr ,
        :md ,
        :mp ,
        :nc ,
        :o-r ,
        :oc ,
        :od ,
        :or ,
        :p-ar ,
        :p-crl ,
        :p-d ,
        :pa ,
        :pg ,
        :psbg ,
        :r-rr ,
        :r-sfr ,
        :rrn ,
        :s-m ,
        :s211 ,
        :sar ,
        :schp ,
        :sd ,
        :sdg ,
        :sfw ,
        :sp ,
        :sr ,
        :ta-c ,
        :tac ,
        :tacpi ,
        :ts ,
        :uevc ,
        :wbr ,
        :wi-d ;
    skos:historyNote """2025-05 NJC: Added status experimental""" ;
    skos:prefLabel "NZ types of Survey Documentation" ;
    skos:scopeNote "termtype:DocType" ;
    schema:creator <https://linked.data.gov.au/org/csdm-pg> ;
    schema:dateCreated "2022-03-18"^^xsd:date ;
    schema:dateModified "2025-05-23"^^xsd:date ;
    schema:keywords unggim:LandParcels ;
    schema:publisher <https://linked.data.gov.au/org/icsm> ;
    schema:status <https://linked.data.gov.au/def/reg-statuses/experimental> ;
.

[]    a prov:Activity ;
    prov:endedAtTime "2024-04-11T06:11:33.572674"^^xsd:dateTime ;
    prov:startedAtTime "2024-04-11T06:11:33.435788"^^xsd:dateTime ;
    prov:used
        [
            a prov:Entity ;
            dcterms:format "application/json" ;
            dcterms:hasVersion "git:29bbdd91c50914400e0758872364ec1cea2d1501" ;
            rdfs:seeAlso "file:///home/runner/work/icsm-vocabs/icsm-vocabs/cadastre/CSD-Header/nz-survey-documentation-type.csv" ;
        ] ;
    prov:wasAssociatedWith
        [
            a
                prov:Agent ,
                schema:SoftwareApplication ;
            rdfs:label "OGC-NA tools" ;
            dcterms:hasVersion "0.3.44" ;
            rdfs:seeAlso "https://github.com/opengeospatial/ogc-na-tools" ;
        ] ;
    prov:wasInformedBy
        [
            dcterms:identifier "42611fe7-ad51-40e1-adf8-e3a0f1ee7a83" ;
        ] ;
.
