PREFIX : <https://linked.data.gov.au/def/csdm/icsm-distance-type/>
PREFIX cs: <https://linked.data.gov.au/def/csdm/icsm-distance-type>
PREFIX dct: <http://purl.org/dc/terms/>
PREFIX prov: <http://www.w3.org/ns/prov#>
PREFIX rdfs: <http://www.w3.org/2000/01/rdf-schema#>
PREFIX schema: <https://schema.org/>
PREFIX skos: <http://www.w3.org/2004/02/skos/core#>
PREFIX surv: <https://linked.data.gov.au/def/csdm/surveyfeatures/>
PREFIX xsd: <http://www.w3.org/2001/XMLSchema#>

:3d-vector
    a
        skos:Concept ,
        surv:Distance ;
    skos:altLabel "Slope" ;
    skos:definition "The reduced observed slope distance between two survey marks." ;
    skos:inScheme cs: ;
    skos:notation "3d-vector" ;
    skos:prefLabel "3D Vector" ;
    skos:topConceptOf cs: ;
.

:ellipsoid
    a
        skos:Concept ,
        surv:Distance ;
    skos:definition "The minimal length of a curve that joins two survey marks on a reference ellipsoid" ;
    skos:inScheme cs: ;
    skos:notation "ellipsoid" ;
    skos:prefLabel "Ellipsoid" ;
    skos:topConceptOf cs: ;
.

:geodetic
    a
        skos:Concept ,
        surv:Distance ;
    skos:definition "The minimal length of a curve that joins two survey marks on a geodetic reference ellipsoid" ;
    skos:inScheme cs: ;
    skos:notation "geodetic" ;
    skos:prefLabel "Geodetic" ;
    skos:topConceptOf cs: ;
.

:ground
    a
        skos:Concept ,
        surv:Distance ;
    skos:altLabel "G" ;
    skos:definition "The reduced observed distance between two survey marks at ground level" ;
    skos:inScheme cs: ;
    skos:notation "ground" ;
    skos:prefLabel "Ground" ;
    skos:topConceptOf cs: ;
.

:horizontal
    a
        skos:Concept ,
        surv:Distance ;
    skos:definition "The reduced observed distance between two survey marks further reduced to a horizontal plane" ;
    skos:inScheme cs: ;
    skos:notation "horizontal" ;
    skos:prefLabel "Horizontal" ;
    skos:topConceptOf cs: ;
.

:mean-elevation
    a
        skos:Concept ,
        surv:Distance ;
    skos:altLabel "Horizontal ground distance at mean elevation" ;
    skos:definition " The reduced observed horizontal distance between two survey marks adjusted to the mean elevation of the line measured" ;
    skos:inScheme cs: ;
    skos:notation "mean-elevation" ;
    skos:prefLabel "Mean Elevation" ;
    skos:topConceptOf cs: ;
.

:slope
    a
        skos:Concept ,
        surv:Distance ;
    skos:definition "The reduced observed distance between two survey marks at ground level" ;
    skos:inScheme cs: ;
    skos:notation "slope" ;
    skos:prefLabel "Slope" ;
    skos:topConceptOf cs: ;
.

:spheroid
    a
        skos:Concept ,
        surv:Distance ;
    skos:altLabel "S" ;
    skos:definition "The shortest distance between two points along the surface of a reference spheroid" ;
    skos:inScheme cs: ;
    skos:notation "spheroid" ;
    skos:prefLabel "Spheroid" ;
    skos:topConceptOf cs: ;
.

<https://linked.data.gov.au/org/csdm-pg>
    a schema:Organization ;
    schema:name "CSDM Project Group" ;
    schema:parentOrganization <https://linked.data.gov.au/org/icsm> ;
    schema:url "https://icsm-au.github.io/3d-csdm/docs/"^^xsd:anyURI ;
.

<https://linked.data.gov.au/org/icsm>
    a schema:Organization ;
    schema:name "Intergovernmental Committee on Surveying & Mapping" ;
    schema:url "https://icsm.gov.au"^^xsd:anyURI ;
.

cs:
    a skos:ConceptScheme ;
    skos:definition "ICSM Distance Type"@en ;
    skos:hasTopConcept
        :3d-vector ,
        :ellipsoid ,
        :geodetic ,
        :ground ,
        :horizontal ,
        :mean-elevation ,
        :slope ,
        :spheroid ;
    skos:prefLabel "ICSM Distance Type" ;
    skos:scopeNote "surv:Distance" ;
    schema:creator <https://linked.data.gov.au/org/csdm-pg> ;
    schema:dateCreated "2022-03-18"^^xsd:date ;
    schema:dateModified "2024-08-20"^^xsd:date ;
    schema:keywords <https://linked.data.gov.au/def/unggim-themes/LandParcels> ;
    schema:publisher <https://linked.data.gov.au/org/icsm> ;
.

[]    a prov:Activity ;
    prov:endedAtTime "2024-04-11T06:11:40.930118"^^xsd:dateTime ;
    prov:startedAtTime "2024-04-11T06:11:40.860549"^^xsd:dateTime ;
    prov:used
        [
            a prov:Entity ;
            dct:format "application/json" ;
            dct:hasVersion "git:29bbdd91c50914400e0758872364ec1cea2d1501" ;
            rdfs:seeAlso <file:///home/runner/work/icsm-vocabs/icsm-vocabs/cadastre/SurveyObservations/icsm-distance-type.csv> ;
        ] ;
    prov:wasAssociatedWith
        [
            a
                prov:Agent ,
                schema:SoftwareApplication ;
            rdfs:label "OGC-NA tools" ;
            dct:hasVersion "0.3.44" ;
            rdfs:seeAlso <https://github.com/opengeospatial/ogc-na-tools> ;
        ] ;
    prov:wasInformedBy
        [
            dct:identifier "42611fe7-ad51-40e1-adf8-e3a0f1ee7a83" ;
        ] ; ;
.
