PREFIX : <https://linked.data.gov.au/def/csdm/icsm-angle-type/>
PREFIX cs: <https://linked.data.gov.au/def/csdm/icsm-angle-type>
PREFIX dcterms: <http://purl.org/dc/terms/>
PREFIX prov: <http://www.w3.org/ns/prov#>
PREFIX rdfs: <http://www.w3.org/2000/01/rdf-schema#>
PREFIX schema: <https://schema.org/>
PREFIX skos: <http://www.w3.org/2004/02/skos/core#>
PREFIX surv: <https://linked.data.gov.au/def/csdm/surveyfeatures/>
PREFIX unggim: <https://linked.data.gov.au/def/unggim-themes/>
PREFIX xsd: <http://www.w3.org/2001/XMLSchema#>

:angle
    a
        skos:Concept ,
        surv:Angle ;
    skos:definition "The acute horizontal angle measured from a reference vector to the observed vector" ;
    skos:inScheme cs: ;
    skos:notation "angle" ;
    skos:prefLabel "Angle" ;
    skos:topConceptOf cs: ;
.

:azimuth
    a
        skos:Concept ,
        surv:Angle ;
    skos:definition "The horizontal angle measured clockwise from any reference meridian to the observed vector" ;
    skos:inScheme cs: ;
    skos:notation "azimuth" ;
    skos:prefLabel "Azimuth" ;
    skos:topConceptOf cs: ;
.

:bearing
    a
        skos:Concept ,
        surv:Angle ;
    skos:definition "The horizontal angle measured clockwise from the CRS meridian to the observed vector" ;
    skos:inScheme cs: ;
    skos:notation "bearing" ;
    skos:prefLabel "Bearing" ;
    skos:topConceptOf cs: ;
.

:mid-azimuth
    a
        skos:Concept ,
        surv:Angle ;
    skos:definition "The mean of the forward azimuth at the start of the line and the reverse azimuth at the end of the line" ;
    skos:inScheme cs: ;
    skos:notation "mid-azimuth" ;
    skos:prefLabel "Mid-azimuth" ;
    skos:topConceptOf cs: ;
.

:subtended
    a
        skos:Concept ,
        surv:Angle ;
    skos:definition "A subtended angle is an angle formed by two lines, or line segments that originate from the same point and extend to two different points on a circle's circumference." ;
    skos:inScheme cs: ;
    skos:notation "subtended" ;
    skos:prefLabel "Subtended" ;
    skos:topConceptOf cs: ;
.

:v-angle
    a
        skos:Concept ,
        surv:Angle ;
    skos:definition "The vertical angle measured from the horizontal plane to the observed vector" ;
    skos:inScheme cs: ;
    skos:notation "v-angle" ;
    skos:prefLabel "Vertical Angle" ;
    skos:topConceptOf cs: ;
.

<https://linked.data.gov.au/org/csdm-pg>
    a schema:Organization ;
    schema:name "CSDM Project Group" ;
    schema:parentOrganization <https://linked.data.gov.au/org/icsm> ;
    schema:url "https://icsm-au.github.io/3d-csdm/docs/"^^xsd:anyURI ;
.

cs:
    a skos:ConceptScheme ;
    skos:definition "ICSM Angle Types"@en ;
    skos:hasTopConcept
        :angle ,
        :azimuth ,
        :bearing ,
        :mid-azimuth ,
        :subtended ,
        :v-angle ;
    skos:prefLabel "ICSM Angle Types" ;
    skos:scopeNote "surv:Angle" ;
    schema:creator <https://linked.data.gov.au/org/csdm-pg> ;
    schema:dateCreated "2022-03-18"^^xsd:date ;
    schema:dateModified "2024-08-20"^^xsd:date ;
    schema:keywords unggim:LandParcels ;
    schema:publisher <https://linked.data.gov.au/org/icsm> ;
.

[]    a prov:Activity ;
    prov:endedAtTime "2024-04-11T06:11:34.659782"^^xsd:dateTime ;
    prov:startedAtTime "2024-04-11T06:11:34.591944"^^xsd:dateTime ;
    prov:used
        [
            a prov:Entity ;
            dcterms:format "application/json" ;
            dcterms:hasVersion "git:29bbdd91c50914400e0758872364ec1cea2d1501" ;
            rdfs:seeAlso "file:///home/runner/work/icsm-vocabs/icsm-vocabs/cadastre/SurveyObservations/icsm-angle-type.csv" ;
        ] ;
    prov:wasAssociatedWith
        [
            a
                prov:Agent ,
                schema:SoftwareApplication ;
            rdfs:label "OGC-NA tools" ;
            dcterms:hasVersion "0.3.44" ;
            rdfs:seeAlso "https://github.com/opengeospatial/ogc-na-tools" ;
        ] ;
    prov:wasInformedBy
        [
            dcterms:identifier "42611fe7-ad51-40e1-adf8-e3a0f1ee7a83" ;
        ] ;
.
