PREFIX : <https://linked.data.gov.au/def/csdm/nz-secondary-purpose/>
PREFIX cs: <https://linked.data.gov.au/def/csdm/nz-secondary-purpose>
PREFIX dct: <http://purl.org/dc/terms/>
PREFIX prov: <http://www.w3.org/ns/prov#>
PREFIX rdfs: <http://www.w3.org/2000/01/rdf-schema#>
PREFIX schema: <https://schema.org/>
PREFIX skos: <http://www.w3.org/2004/02/skos/core#>
PREFIX termtype: <https://linked.data.gov.au/def/csdm/termtypes/>
PREFIX xsd: <http://www.w3.org/2001/XMLSchema#>

:prow
    a
        skos:Concept ,
        termtype:ParcelPurpose ;
    skos:definition "A right held by the Dominant Tenement (Benefited Land) to walk upon the Servient Tenement (Burdened Land) as a means of access to or egress from the Dominant Tenement" ;
    skos:inScheme cs: ;
    skos:notation "prow" ;
    skos:prefLabel "Pedestrian Right of Way" ;
    skos:topConceptOf cs: ;
.

:r-ct
    a
        skos:Concept ,
        termtype:ParcelPurpose ;
    skos:definition "A right held by the Dominant Tenement (Benefited Land) to use the Servient Tenement (Burdened Land) to convey electricity and electrical telecommunications without interruption or impediment" ;
    skos:inScheme cs: ;
    skos:notation "r-ct" ;
    skos:prefLabel "Right to convey Telecommunications" ;
    skos:topConceptOf cs: ;
.

:rce
    a
        skos:Concept ,
        termtype:ParcelPurpose ;
    skos:definition "A right held by the Dominant Tenement (Benefited Land) to use the Servient Tenement (Burdened Land) to convey electricity and electrical impulses without interruption or impediment" ;
    skos:inScheme cs: ;
    skos:notation "rce" ;
    skos:prefLabel "Right to convey Electricity" ;
    skos:topConceptOf cs: ;
.

:rcg
    a
        skos:Concept ,
        termtype:ParcelPurpose ;
    skos:definition "A right held by the Dominant Tenement (Benefited Land) to use the Servient Tenement (Burdened Land) to convey gas without interruption or impediment" ;
    skos:inScheme cs: ;
    skos:notation "rcg" ;
    skos:prefLabel "Right to convey Gas" ;
    skos:topConceptOf cs: ;
.

:rcm
    a
        skos:Concept ,
        termtype:ParcelPurpose ;
    skos:definition "A right held by the Dominant Tenement (Benefited Land) to use the Servient Tenement (Burdened Land) to convey computer media without interruption or impediment" ;
    skos:inScheme cs: ;
    skos:notation "rcm" ;
    skos:prefLabel "Right to convey Computer Media" ;
    skos:topConceptOf cs: ;
.

:rct-cm
    a
        skos:Concept ,
        termtype:ParcelPurpose ;
    skos:definition "A right held by the Dominant Tenement (Benefited Land) to use the Servient Tenement (Burdened Land) to convey electricity, electrical impulses, and computer media without interruption or impediment" ;
    skos:inScheme cs: ;
    skos:notation "rct-cm" ;
    skos:prefLabel "Right to convey Telecommunications and Computer Media" ;
    skos:topConceptOf cs: ;
.

:rcw
    a
        skos:Concept ,
        termtype:ParcelPurpose ;
    skos:definition "A right held by the Dominant Tenement (Benefited Land) to use the Servient Tenement (Burdened Land) to convey water in free and unimpeded flow without interruption or impediment" ;
    skos:inScheme cs: ;
    skos:notation "rcw" ;
    skos:prefLabel "Right to convey Water" ;
    skos:topConceptOf cs: ;
.

:rds
    a
        skos:Concept ,
        termtype:ParcelPurpose ;
    skos:definition "A right held by the Dominant Tenement (Benefited Land) to use the Servient Tenement (Burdened Land) to drain, discharge, and convey sewage and other waste material and waste fluids in any quantity without interruption or impediment" ;
    skos:inScheme cs: ;
    skos:notation "rds" ;
    skos:prefLabel "Right to drain Sewage" ;
    skos:topConceptOf cs: ;
.

:rdsw
    a
        skos:Concept ,
        termtype:ParcelPurpose ;
    skos:definition "A right held by the Dominant Tenement (Benefited Land) to use the Servient Tenement (Burdened Land) to convey storm water in any quantity without interruption or impediment" ;
    skos:inScheme cs: ;
    skos:notation "rdsw" ;
    skos:prefLabel "Right to drain Storm Water" ;
    skos:topConceptOf cs: ;
.

:rdw
    a
        skos:Concept ,
        termtype:ParcelPurpose ;
    skos:definition "A right held by the Dominant Tenement (Benefited Land) to use the Servient Tenement (Burdened Land) to convey water (whether sourced from rain, springs, soakage, or seepage) in any quantity without interruption or impediment" ;
    skos:inScheme cs: ;
    skos:notation "rdw" ;
    skos:prefLabel "Right to drain Water" ;
    skos:topConceptOf cs: ;
.

:red
    a
        skos:Concept ,
        termtype:ParcelPurpose ;
    skos:definition "A right held by the Dominant Tenement (Benefited Land) to emit dust" ;
    skos:inScheme cs: ;
    skos:notation "red" ;
    skos:prefLabel "Right to emit Dust" ;
    skos:topConceptOf cs: ;
.

:ren
    a
        skos:Concept ,
        termtype:ParcelPurpose ;
    skos:definition "A right held by the Dominant Tenement (Benefited Land) to emit noise" ;
    skos:inScheme cs: ;
    skos:notation "ren" ;
    skos:prefLabel "Right to emit Noise" ;
    skos:topConceptOf cs: ;
.

:res
    a
        skos:Concept ,
        termtype:ParcelPurpose ;
    skos:definition "A right held by the Dominant Tenement (Benefited Land) to emit spray" ;
    skos:inScheme cs: ;
    skos:notation "res" ;
    skos:prefLabel "Right to emit Spray" ;
    skos:topConceptOf cs: ;
.

:rl-a
    a
        skos:Concept ,
        termtype:ParcelPurpose ;
    skos:definition "A right held by the Dominant Tenement (Benefited Land) to ensure the Servient Tenement (Burdened Land) provides unobstructed access to light and air" ;
    skos:inScheme cs: ;
    skos:notation "rl-a" ;
    skos:prefLabel "Right to Light and Air" ;
    skos:topConceptOf cs: ;
.

:roe
    a
        skos:Concept ,
        termtype:ParcelPurpose ;
    skos:definition "A right held by the Dominant Tenement (Benefited Land) to allow eaves to encroach over the Servient Tenement (Burdened Land)" ;
    skos:inScheme cs: ;
    skos:notation "roe" ;
    skos:prefLabel "Right to Overhang Eaves" ;
    skos:topConceptOf cs: ;
.

:row
    a
        skos:Concept ,
        termtype:ParcelPurpose ;
    skos:definition "A right held by the Dominant Tenement (Benefited Land) to use the Servient Tenement (Burdened Land) as a means of access to or egress from the Dominant Tenement" ;
    skos:inScheme cs: ;
    skos:notation "row" ;
    skos:prefLabel "Rights of Way" ;
    skos:topConceptOf cs: ;
.

:rp
    a
        skos:Concept ,
        termtype:ParcelPurpose ;
    skos:definition "A right held by the Dominant Tenement (Benefited Land) to use the Servient Tenement (Burdened Land) to park vehicles without interruption or impediment" ;
    skos:inScheme cs: ;
    skos:notation "rp" ;
    skos:prefLabel "Right to Parking" ;
    skos:topConceptOf cs: ;
.

:rs
    a
        skos:Concept ,
        termtype:ParcelPurpose ;
    skos:definition "A right held by the Dominant Tenement (Benefited Land) to require the Servient Tenement (Burdened Land) to ensure structures on the Dominant Tenement are supported" ;
    skos:inScheme cs: ;
    skos:notation "rs" ;
    skos:prefLabel "Right to Support" ;
    skos:topConceptOf cs: ;
.

<https://linked.data.gov.au/org/csdm-pg>
    a schema:Organization ;
    schema:name "CSDM Project Group" ;
    schema:parentOrganization <https://linked.data.gov.au/org/icsm> ;
    schema:url "https://icsm-au.github.io/3d-csdm/docs/"^^xsd:anyURI ;
.

<https://linked.data.gov.au/org/icsm>
    a schema:Organization ;
    schema:name "Intergovernmental Committee on Surveying & Mapping" ;
    schema:url "https://icsm.gov.au"^^xsd:anyURI ;
.

cs:
    a skos:ConceptScheme ;
    skos:definition "NZ Secondary Purpose"@en ;
    skos:hasTopConcept
        :prow ,
        :r-ct ,
        :rce ,
        :rcg ,
        :rcm ,
        :rct-cm ,
        :rcw ,
        :rds ,
        :rdsw ,
        :rdw ,
        :red ,
        :ren ,
        :res ,
        :rl-a ,
        :roe ,
        :row ,
        :rp ,
        :rs ;
    skos:prefLabel "NZ Secondary Purpose" ;
    skos:scopeNote "termtype:ParcelPurpose" ;
    schema:creator <https://linked.data.gov.au/org/csdm-pg> ;
    schema:dateCreated "2022-03-18"^^xsd:date ;
    schema:dateModified "2024-04-11"^^xsd:date ;
    schema:publisher <https://linked.data.gov.au/org/icsm> ;
.

[]    a prov:Activity ;
    prov:endedAtTime "2024-04-11T06:11:40.855354"^^xsd:dateTime ;
    prov:startedAtTime "2024-04-11T06:11:40.777071"^^xsd:dateTime ;
    prov:used
        [
            a prov:Entity ;
            dct:format "application/json" ;
            dct:hasVersion "git:29bbdd91c50914400e0758872364ec1cea2d1501" ;
            rdfs:seeAlso <file:///home/runner/work/icsm-vocabs/icsm-vocabs/cadastre/Parcels/nz-secondary-purpose.csv> ;
        ] ;
    prov:wasAssociatedWith
        [
            a
                prov:Agent ,
                schema:SoftwareApplication ;
            rdfs:label "OGC-NA tools" ;
            dct:hasVersion "0.3.44" ;
            rdfs:seeAlso <https://github.com/opengeospatial/ogc-na-tools> ;
        ] ;
    prov:wasInformedBy
        [
            dct:identifier "42611fe7-ad51-40e1-adf8-e3a0f1ee7a83" ;
        ] ; ;
.
