PREFIX : <https://linked.data.gov.au/def/csdm/icsm-parcel-state/>
PREFIX cs: <https://linked.data.gov.au/def/csdm/icsm-parcel-state>
PREFIX dct: <http://purl.org/dc/terms/>
PREFIX prov: <http://www.w3.org/ns/prov#>
PREFIX rdfs: <http://www.w3.org/2000/01/rdf-schema#>
PREFIX schema: <https://schema.org/>
PREFIX skos: <http://www.w3.org/2004/02/skos/core#>
PREFIX termtype: <https://linked.data.gov.au/def/csdm/termtypes/>
PREFIX xsd: <http://www.w3.org/2001/XMLSchema#>

:a
    a
        skos:Concept ,
        termtype:ParcelState ;
    skos:definition "The parcel must be amalgamated with one or more parcels created by the survey when the survey is deposited" ;
    skos:inScheme cs: ;
    skos:notation "a" ;
    skos:prefLabel "affected" ;
    skos:topConceptOf cs: ;
.

:affected-tenure
    a
        skos:Concept ,
        termtype:ParcelState ;
    skos:definition "Document state: The parcel is to be encumbured" ;
    skos:inScheme cs: ;
    skos:notation "affected-tenure" ;
    skos:prefLabel "affected tenure" ;
    skos:topConceptOf cs: ;
.

:c
    a
        skos:Concept ,
        termtype:ParcelState ;
    skos:definition "The parcel is being created by the survey" ;
    skos:inScheme cs: ;
    skos:notation "c" ;
    skos:prefLabel "created" ;
    skos:topConceptOf cs: ;
.

:cancelled
    a
        skos:Concept ,
        termtype:ParcelState ;
    skos:definition "Document and Database State: Plan/Scheme unregistered and cancelled" ;
    skos:inScheme cs: ;
    skos:notation "cancelled" ;
    skos:prefLabel "cancelled" ;
    skos:topConceptOf cs: ;
.

:enc
    a
        skos:Concept ,
        termtype:ParcelState ;
    skos:definition "The parcel has been subject to natural erosion and/or accretion and the definition of the parcel has been/should be updated. Relevant where the parcel affected by the accretion/erosion is not extinguished by the survey" ;
    skos:inScheme cs: ;
    skos:notation "enc" ;
    skos:prefLabel "encroached" ;
    skos:topConceptOf cs: ;
.

:exist
    a
        skos:Concept ,
        termtype:ParcelState ;
    skos:definition "The parcel is referenced by the survey" ;
    skos:inScheme cs: ;
    skos:notation "exist" ;
    skos:prefLabel "existing" ;
    skos:topConceptOf cs: ;
.

:exting
    a
        skos:Concept ,
        termtype:ParcelState ;
    skos:definition "The parcel is being replaced by one or more parcels created by the survey" ;
    skos:inScheme cs: ;
    skos:notation "exting" ;
    skos:prefLabel "extinguished" ;
    skos:topConceptOf cs: ;
.

:former-tenure
    a
        skos:Concept ,
        termtype:ParcelState ;
    skos:definition "Document state: The parcel is being replaced by one or more parcels created by the survey" ;
    skos:inScheme cs: ;
    skos:notation "former-tenure" ;
    skos:prefLabel "former tenure" ;
    skos:topConceptOf cs: ;
.

:inset
    a
        skos:Concept ,
        termtype:ParcelState ;
    skos:definition "Document state: The parcel is an inset lot" ;
    skos:inScheme cs: ;
    skos:notation "inset" ;
    skos:prefLabel "inset" ;
    skos:topConceptOf cs: ;
.

:lodged
    a
        skos:Concept ,
        termtype:ParcelState ;
    skos:definition "Database state: Lodged" ;
    skos:inScheme cs: ;
    skos:notation "lodged" ;
    skos:prefLabel "lodged" ;
    skos:topConceptOf cs: ;
.

:prop
    a
        skos:Concept ,
        termtype:ParcelState ;
    skos:definition "The parcel is introduced on the survey but has not actually been ‘created’. This will generally only apply to parcels such as Future Development Units (FDU) on a Proposed Unit Development plan (PUD). The parcel will be created in a subsequent plan, e.g., Stage 1 of the Unit Development" ;
    skos:inScheme cs: ;
    skos:notation "prop" ;
    skos:prefLabel "proposed" ;
    skos:topConceptOf cs: ;
.

:ref
    a
        skos:Concept ,
        termtype:ParcelState ;
    skos:definition "The parcel is referenced by the survey" ;
    skos:inScheme cs: ;
    skos:notation "ref" ;
    skos:prefLabel "referenced" ;
    skos:topConceptOf cs: ;
.

:registered
    a
        skos:Concept ,
        termtype:ParcelState ;
    skos:definition "Database state: Element registered" ;
    skos:inScheme cs: ;
    skos:notation "registered" ;
    skos:prefLabel "registered" ;
    skos:topConceptOf cs: ;
.

:removed
    a
        skos:Concept ,
        termtype:ParcelState ;
    skos:definition "An easement / restriction subject to removal" ;
    skos:inScheme cs: ;
    skos:notation "removed" ;
    skos:prefLabel "removed" ;
    skos:topConceptOf cs: ;
.

:superseded
    a
        skos:Concept ,
        termtype:ParcelState ;
    skos:definition "Database State: Element further subdivided or removed" ;
    skos:inScheme cs: ;
    skos:notation "superseded" ;
    skos:prefLabel "superseded" ;
    skos:topConceptOf cs: ;
.

:terminated
    a
        skos:Concept ,
        termtype:ParcelState ;
    skos:definition "Document and Database State: Plan/Scheme terminated" ;
    skos:inScheme cs: ;
    skos:notation "terminated" ;
    skos:prefLabel "terminated" ;
    skos:topConceptOf cs: ;
.

<https://linked.data.gov.au/org/csdm-pg>
    a schema:Organization ;
    schema:name "CSDM Project Group" ;
    schema:parentOrganization <https://linked.data.gov.au/org/icsm> ;
    schema:url "https://icsm-au.github.io/3d-csdm/docs/"^^xsd:anyURI ;
.

<https://linked.data.gov.au/org/icsm>
    a schema:Organization ;
    schema:name "Intergovernmental Committee on Surveying & Mapping" ;
    schema:url "https://icsm.gov.au"^^xsd:anyURI ;
.

cs:
    a skos:ConceptScheme ;
    skos:definition "ICSM Parcel State"@en ;
    skos:hasTopConcept
        :a ,
        :affected-tenure ,
        :c ,
        :cancelled ,
        :enc ,
        :exist ,
        :exting ,
        :former-tenure ,
        :inset ,
        :lodged ,
        :prop ,
        :ref ,
        :registered ,
        :removed ,
        :superseded ,
        :terminated ;
    skos:prefLabel "ICSM Parcel State" ;
    skos:scopeNote "termtype:ParcelState" ;
    schema:creator <https://linked.data.gov.au/org/csdm-pg> ;
    schema:dateCreated "2022-03-18"^^xsd:date ;
    schema:dateModified "2024-04-11"^^xsd:date ;
    schema:publisher <https://linked.data.gov.au/org/icsm> ;
.

[]    a prov:Activity ;
    prov:endedAtTime "2024-04-11T06:11:42.830934"^^xsd:dateTime ;
    prov:startedAtTime "2024-04-11T06:11:42.754445"^^xsd:dateTime ;
    prov:used
        [
            a prov:Entity ;
            dct:format "application/json" ;
            dct:hasVersion "git:29bbdd91c50914400e0758872364ec1cea2d1501" ;
            rdfs:seeAlso <file:///home/runner/work/icsm-vocabs/icsm-vocabs/cadastre/Parcels/icsm-parcel-state.csv> ;
        ] ;
    prov:wasAssociatedWith
        [
            a
                prov:Agent ,
                schema:SoftwareApplication ;
            rdfs:label "OGC-NA tools" ;
            dct:hasVersion "0.3.44" ;
            rdfs:seeAlso <https://github.com/opengeospatial/ogc-na-tools> ;
        ] ;
    prov:wasInformedBy
        [
            dct:identifier "42611fe7-ad51-40e1-adf8-e3a0f1ee7a83" ;
        ] ; ;
.
