PREFIX : <https://linked.data.gov.au/def/csdm/vic-parcel-state/>
PREFIX cs: <https://linked.data.gov.au/def/csdm/vic-parcel-state>
PREFIX dcterms: <http://purl.org/dc/terms/>
PREFIX prov: <http://www.w3.org/ns/prov#>
PREFIX rdfs: <http://www.w3.org/2000/01/rdf-schema#>
PREFIX schema: <https://schema.org/>
PREFIX skos: <http://www.w3.org/2004/02/skos/core#>
PREFIX termtype: <https://linked.data.gov.au/def/csdm/termtypes/>
PREFIX unggim: <https://linked.data.gov.au/def/unggim-themes/>
PREFIX xsd: <http://www.w3.org/2001/XMLSchema#>

:affected
    a
        skos:Concept ,
        termtype:ParcelState ;
    skos:definition "An existing parcel subject to amendment due to new boundary adoption from an abutting parcel" ;
    skos:inScheme cs: ;
    skos:notation "affected" ;
    skos:prefLabel "Affected" ;
    skos:topConceptOf cs: ;
.

:cancelled
    a
        skos:Concept ,
        termtype:ParcelState ;
    skos:definition "An existing parcel subject to cancellation" ;
    skos:inScheme cs: ;
    skos:notation "cancelled" ;
    skos:prefLabel "Cancelled" ;
    skos:topConceptOf cs: ;
.

:created
    a
        skos:Concept ,
        termtype:ParcelState ;
    skos:definition "A new parcel being created in a plan (e.g. (PS) plan of subdivision; (OP) original plan" ;
    skos:inScheme cs: ;
    skos:notation "created" ;
    skos:prefLabel "Created" ;
    skos:topConceptOf cs: ;
.

:encroached
    a
        skos:Concept ,
        termtype:ParcelState ;
    skos:definition "An existing parcel encroached by a new boundary adoption from an abutting parcel" ;
    skos:inScheme cs: ;
    skos:notation "encroached" ;
    skos:prefLabel "Encroached" ;
    skos:topConceptOf cs: ;
.

:existing
    a
        skos:Concept ,
        termtype:ParcelState ;
    skos:definition "A parcel that exists on the cadastre and the boundaries are not affected" ;
    skos:inScheme cs: ;
    skos:notation "existing" ;
    skos:prefLabel "Existing" ;
    skos:topConceptOf cs: ;
.

:removed
    a
        skos:Concept ,
        termtype:ParcelState ;
    skos:definition "An easement / restriction subject to removal" ;
    skos:inScheme cs: ;
    skos:notation "removed" ;
    skos:prefLabel "Removed" ;
    skos:topConceptOf cs: ;
.

cs:
    a skos:ConceptScheme ;
    skos:definition "VIC Parcel State"@en ;
    skos:hasTopConcept
        :affected ,
        :cancelled ,
        :created ,
        :encroached ,
        :existing ,
        :removed ;
    skos:historyNote """2025-05 NJC: Added status experimental""" ;
    skos:prefLabel "VIC Parcel State" ;
    skos:scopeNote "termtype:ParcelState" ;
    schema:creator <https://linked.data.gov.au/org/csdm-pg> ;
    schema:dateCreated "2022-03-18"^^xsd:date ;
    schema:dateModified "2025-05-22"^^xsd:date ;
    schema:keywords unggim:LandParcels ;
    schema:publisher <https://linked.data.gov.au/org/icsm> ;
    schema:status <https://linked.data.gov.au/def/reg-statuses/experimental> ;
.

[]    a prov:Activity ;
    prov:endedAtTime "2024-04-11T06:11:34.949529"^^xsd:dateTime ;
    prov:startedAtTime "2024-04-11T06:11:34.881056"^^xsd:dateTime ;
    prov:used
        [
            a prov:Entity ;
            dcterms:format "application/json" ;
            dcterms:hasVersion "git:29bbdd91c50914400e0758872364ec1cea2d1501" ;
            rdfs:seeAlso "file:///home/runner/work/icsm-vocabs/icsm-vocabs/cadastre/Parcels/vic-parcel-state.csv" ;
        ] ;
    prov:wasAssociatedWith
        [
            a
                prov:Agent ,
                schema:SoftwareApplication ;
            rdfs:label "OGC-NA tools" ;
            dcterms:hasVersion "0.3.44" ;
            rdfs:seeAlso "https://github.com/opengeospatial/ogc-na-tools" ;
        ] ;
    prov:wasInformedBy
        [
            dcterms:identifier "42611fe7-ad51-40e1-adf8-e3a0f1ee7a83" ;
        ] ;
.
